<?xml version="1.0"?>
<rdf:RDF xmlns="http://www.esonetyellowpages.com/vocab/"
     xml:base="http://www.esonetyellowpages.com/vocab/"
     xmlns:schema="http://schema.org/"
     xmlns:rdf="http://www.w3.org/1999/02/22-rdf-syntax-ns#"
     xmlns:owl="http://www.w3.org/2002/07/owl#"
     xmlns:xml="http://www.w3.org/XML/1998/namespace"
     xmlns:xsd="http://www.w3.org/2001/XMLSchema#"
     xmlns:rdfs="http://www.w3.org/2000/01/rdf-schema#"
     xmlns:dc="http://purl.org/dc/elements/1.1/"
     xmlns:ssn="https://www.w3.org/ns/ssn/">
    <owl:Ontology rdf:about="http://www.esonetyellowpages.com/vocab/">
        <dc:date>2016-08-01</dc:date>
        <dc:title>ESONET Yellow Pages Ontology</dc:title>
        <dc:creator>Markus Stocker</dc:creator>
        <rdfs:comment rdf:datatype="http://www.w3.org/2001/XMLSchema#string">This ontology is based on the SSN Ontology by the W3C Semantic Sensor Networks Incubator Group (SSN-XG).</rdfs:comment>
        <rdfs:comment>New modular version of the SSN ontology independent of DUL.</rdfs:comment>
        <dc:title>Semantic Sensor Network Ontology</dc:title>
        <rdfs:seeAlso rdf:datatype="http://www.w3.org/2001/XMLSchema#anyURI">http://www.esonetyellowpages.com/</rdfs:seeAlso>
        <owl:versionInfo>0.1</owl:versionInfo>
        <rdfs:comment rdf:datatype="http://www.w3.org/2001/XMLSchema#string">This ontology describes sensors and observations, and related concepts. It does not describe domain concepts, time, locations, etc. as these are intended to be included from other ontologies via OWL imports.</rdfs:comment>
    </owl:Ontology>
    


    <!-- 
    ///////////////////////////////////////////////////////////////////////////////////////
    //
    // Annotation properties
    //
    ///////////////////////////////////////////////////////////////////////////////////////
     -->

    


    <!-- http://purl.org/dc/elements/1.1/source -->

    <owl:AnnotationProperty rdf:about="http://purl.org/dc/elements/1.1/source"/>
    


    <!-- http://purl.org/dc/elements/1.1/title -->

    <owl:AnnotationProperty rdf:about="http://purl.org/dc/elements/1.1/title"/>
    


    <!-- 
    ///////////////////////////////////////////////////////////////////////////////////////
    //
    // Object Properties
    //
    ///////////////////////////////////////////////////////////////////////////////////////
     -->

    


    <!-- http://schema.org/unitCode -->

    <rdf:Description rdf:about="http://schema.org/unitCode">
        <rdfs:comment xml:lang="en">The unit of measurement given using the UN/CEFACT Common Code (3 characters) or a URL. Other codes than the UN/CEFACT Common Code may be used with a prefix followed by a colon.</rdfs:comment>
        <rdfs:label xml:lang="en">unit code</rdfs:label>
    </rdf:Description>
    


    <!-- http://www.w3.org/2002/07/owl#topObjectProperty -->

    <rdf:Description rdf:about="http://www.w3.org/2002/07/owl#topObjectProperty">
        <rdf:type rdf:resource="http://www.w3.org/2002/07/owl#SymmetricProperty"/>
        <rdf:type rdf:resource="http://www.w3.org/2002/07/owl#TransitiveProperty"/>
        <rdf:type rdf:resource="http://www.w3.org/2002/07/owl#ReflexiveProperty"/>
    </rdf:Description>
    


    <!-- https://www.w3.org/ns/ssn/attachedSystem -->

    <owl:ObjectProperty rdf:about="https://www.w3.org/ns/ssn/attachedSystem">
        <owl:inverseOf rdf:resource="https://www.w3.org/ns/ssn/onPlatform"/>
        <rdfs:comment>Relation between a Platform and any Systems (e.g., Sensors) that are attached to the Platform.</rdfs:comment>
        <rdfs:label>attached system</rdfs:label>
    </owl:ObjectProperty>
    


    <!-- https://www.w3.org/ns/ssn/deployedOnPlatform -->

    <owl:ObjectProperty rdf:about="https://www.w3.org/ns/ssn/deployedOnPlatform">
        <owl:inverseOf rdf:resource="https://www.w3.org/ns/ssn/inDeployment"/>
        <rdfs:comment>Relation between a deployment and the platform on which the system was deployed.</rdfs:comment>
        <rdfs:label>deployed on platform</rdfs:label>
    </owl:ObjectProperty>
    


    <!-- https://www.w3.org/ns/ssn/deployedSystem -->

    <owl:ObjectProperty rdf:about="https://www.w3.org/ns/ssn/deployedSystem">
        <owl:inverseOf rdf:resource="https://www.w3.org/ns/ssn/hasDeployment"/>
        <rdfs:comment>Relation between a deployment and the deployed system.</rdfs:comment>
        <rdfs:label>deployed system</rdfs:label>
    </owl:ObjectProperty>
    


    <!-- https://www.w3.org/ns/ssn/deploymentProcessPart -->

    <rdf:Description rdf:about="https://www.w3.org/ns/ssn/deploymentProcessPart">
        <rdfs:comment>Has part relation between a deployment process and its constituent processes.</rdfs:comment>
        <rdfs:label>deployment process part</rdfs:label>
    </rdf:Description>
    


    <!-- https://www.w3.org/ns/ssn/detects -->

    <rdf:Description rdf:about="https://www.w3.org/ns/ssn/detects">
        <rdfs:comment>A relation from a sensor to the Stimulus that the sensor can detect.   
The Stimulus itself will be serving as a proxy for (see isProxyOf) some observable property.</rdfs:comment>
        <rdfs:label>detects</rdfs:label>
    </rdf:Description>
    


    <!-- https://www.w3.org/ns/ssn/featureInObservation -->

    <owl:ObjectProperty rdf:about="https://www.w3.org/ns/ssn/featureInObservation">
        <rdfs:subPropertyOf rdf:resource="http://www.w3.org/2002/07/owl#topObjectProperty"/>
        <owl:inverseOf rdf:resource="https://www.w3.org/ns/ssn/featureOfInterest"/>
    </owl:ObjectProperty>
    


    <!-- https://www.w3.org/ns/ssn/featureOfInterest -->

    <owl:ObjectProperty rdf:about="https://www.w3.org/ns/ssn/featureOfInterest">
        <dc:source>skos:exactMatch &apos;featureOfInterest&apos; [O&amp;M - ISO/DIS 19156] 
		                    http://portal.opengeospatial.org/files/?artifact_id=41579</dc:source>
        <rdfs:comment>A relation between an observation and the entity whose quality was observed.   For example, in an observation of the weight of a person, the feature of interest is the person and the quality is weight.</rdfs:comment>
        <rdfs:label>feature of interest</rdfs:label>
    </owl:ObjectProperty>
    


    <!-- https://www.w3.org/ns/ssn/forProperty -->

    <rdf:Description rdf:about="https://www.w3.org/ns/ssn/forProperty">
        <rdfs:comment>A relation between some aspect of a sensing entity and a property.  For example, from a sensor to the properties it can observe, or from a deployment to the properties it was installed to observe.  Also from a measurement capability to the property the capability is described for.  (Used in conjunction with ofFeature).</rdfs:comment>
        <rdfs:label>for property</rdfs:label>
    </rdf:Description>
    


    <!-- https://www.w3.org/ns/ssn/fromStimulus -->

    <rdf:Description rdf:about="https://www.w3.org/ns/ssn/fromStimulus"/>
    


    <!-- https://www.w3.org/ns/ssn/hasDeployment -->

    <owl:ObjectProperty rdf:about="https://www.w3.org/ns/ssn/hasDeployment">
        <rdfs:comment>Relation between a System and a Deployment, recording that the System/Sensor was deployed in that Deployment.</rdfs:comment>
        <rdfs:label>has deployment</rdfs:label>
    </owl:ObjectProperty>
    


    <!-- https://www.w3.org/ns/ssn/hasMeasurementCapability -->

    <owl:ObjectProperty rdf:about="https://www.w3.org/ns/ssn/hasMeasurementCapability">
        <rdfs:subPropertyOf rdf:resource="https://www.w3.org/ns/ssn/hasProperty"/>
        <rdfs:comment>Relation from a Sensor to a MeasurementCapability describing the measurement properties of the sensor.</rdfs:comment>
        <rdfs:label>has measurement capability</rdfs:label>
    </owl:ObjectProperty>
    


    <!-- https://www.w3.org/ns/ssn/hasMeasurementProperty -->

    <owl:ObjectProperty rdf:about="https://www.w3.org/ns/ssn/hasMeasurementProperty">
        <rdfs:subPropertyOf rdf:resource="https://www.w3.org/ns/ssn/hasProperty"/>
        <rdfs:comment>Relation from a MeasurementCapability to a MeasurementProperty.  For example, to an accuracy (see notes at MeasurementCapability).</rdfs:comment>
        <rdfs:label>has measurement property</rdfs:label>
    </owl:ObjectProperty>
    


    <!-- https://www.w3.org/ns/ssn/hasOperatingProperty -->

    <owl:ObjectProperty rdf:about="https://www.w3.org/ns/ssn/hasOperatingProperty">
        <rdfs:subPropertyOf rdf:resource="https://www.w3.org/ns/ssn/hasProperty"/>
        <rdfs:comment>Relation from an OperatingRange to a Property.  For example, to a battery lifetime.</rdfs:comment>
        <rdfs:label>has operating property</rdfs:label>
    </owl:ObjectProperty>
    


    <!-- https://www.w3.org/ns/ssn/hasOperatingRange -->

    <owl:ObjectProperty rdf:about="https://www.w3.org/ns/ssn/hasOperatingRange">
        <rdfs:subPropertyOf rdf:resource="https://www.w3.org/ns/ssn/hasProperty"/>
        <rdfs:comment>Relation from a System to an OperatingRange describing the normal operating environment of the System.</rdfs:comment>
        <rdfs:label>has operating range</rdfs:label>
    </owl:ObjectProperty>
    


    <!-- https://www.w3.org/ns/ssn/hasProperty -->

    <owl:ObjectProperty rdf:about="https://www.w3.org/ns/ssn/hasProperty">
        <owl:inverseOf rdf:resource="https://www.w3.org/ns/ssn/isPropertyOf"/>
        <owl:propertyChainAxiom rdf:parseType="Collection">
            <rdf:Description rdf:about="https://www.w3.org/ns/ssn/featureInObservation"/>
            <rdf:Description rdf:about="https://www.w3.org/ns/ssn/observedProperty"/>
        </owl:propertyChainAxiom>
        <rdfs:comment>A relation between a FeatureOfInterest and a Property of that feature.</rdfs:comment>
        <rdfs:comment>The chain here ensures that the observed property of an observation is a property of the feature of interest.  This restriction is written in O&amp;M; here we can enforce it formally.

The more obvious formulation:

featureOfInterest o hasProperty SubPropertyOf observedProperty

can&apos;t be used, because (by the OWL2 decidability restrictions) that would mean cardinality restrictions couldn&apos;t be applied to observedProperty (see definition of Observation).</rdfs:comment>
        <rdfs:label>has property</rdfs:label>
    </owl:ObjectProperty>
    


    <!-- https://www.w3.org/ns/ssn/hasSubSystem -->

    <rdf:Description rdf:about="https://www.w3.org/ns/ssn/hasSubSystem">
        <rdfs:comment>Haspart relation between a system and its parts.</rdfs:comment>
        <rdfs:label>has subsystem</rdfs:label>
    </rdf:Description>
    


    <!-- https://www.w3.org/ns/ssn/hasSurvivalProperty -->

    <owl:ObjectProperty rdf:about="https://www.w3.org/ns/ssn/hasSurvivalProperty">
        <rdfs:subPropertyOf rdf:resource="https://www.w3.org/ns/ssn/hasProperty"/>
        <rdfs:comment>Relation from a SurvivalRange to a Property describing the survial range of a system.  For example, to the temperature extreme that a system can withstand before being considered damaged.</rdfs:comment>
        <rdfs:label>has survival property</rdfs:label>
    </owl:ObjectProperty>
    


    <!-- https://www.w3.org/ns/ssn/hasSurvivalRange -->

    <owl:ObjectProperty rdf:about="https://www.w3.org/ns/ssn/hasSurvivalRange">
        <rdfs:subPropertyOf rdf:resource="https://www.w3.org/ns/ssn/hasProperty"/>
        <rdfs:comment>A Relation from a System to a SurvivalRange.</rdfs:comment>
        <rdfs:label>has survival range</rdfs:label>
    </owl:ObjectProperty>
    


    <!-- https://www.w3.org/ns/ssn/hasValue -->

    <owl:ObjectProperty rdf:about="https://www.w3.org/ns/ssn/hasValue">
        <owl:inverseOf rdf:resource="https://www.w3.org/ns/ssn/isValueOf"/>
        <rdfs:label>has value</rdfs:label>
    </owl:ObjectProperty>
    


    <!-- https://www.w3.org/ns/ssn/implementedBy -->

    <owl:ObjectProperty rdf:about="https://www.w3.org/ns/ssn/implementedBy">
        <owl:inverseOf rdf:resource="https://www.w3.org/ns/ssn/implements"/>
        <rdfs:comment>A relation between the description of an algorithm, procedure or method and an entity that implements that method in some executable way.  For example, between a scientific measuring method and a sensor the senses via that method.</rdfs:comment>
        <rdfs:label>implemented by</rdfs:label>
    </owl:ObjectProperty>
    


    <!-- https://www.w3.org/ns/ssn/implements -->

    <owl:ObjectProperty rdf:about="https://www.w3.org/ns/ssn/implements">
        <rdfs:comment>A relation between an entity that implements a method in some executable way and the description of an algorithm, procedure or method.  For example, between a Sensor and the scientific measuring method that the Sensor uses to observe a Property.</rdfs:comment>
        <rdfs:label>implements</rdfs:label>
    </owl:ObjectProperty>
    


    <!-- https://www.w3.org/ns/ssn/inCondition -->

    <rdf:Description rdf:about="https://www.w3.org/ns/ssn/inCondition">
        <rdfs:comment>Describes the prevailing environmental conditions for MeasurementCapabilites, OperatingConditions and SurvivalRanges.  Used for example to say that a sensor has a particular accuracy in particular conditions.  (see also MeasurementCapability)</rdfs:comment>
        <rdfs:label>in condition</rdfs:label>
    </rdf:Description>
    


    <!-- https://www.w3.org/ns/ssn/inDeployment -->

    <owl:ObjectProperty rdf:about="https://www.w3.org/ns/ssn/inDeployment">
        <rdfs:comment>Relation between a Platform and a Deployment, recording that the object was used as a platform for a system/sensor for a particular deployment: as in this PhysicalObject is acting as a Platform inDeployment Deployment.</rdfs:comment>
        <rdfs:label>in deployment</rdfs:label>
    </owl:ObjectProperty>
    


    <!-- https://www.w3.org/ns/ssn/isProducedBy -->

    <owl:ObjectProperty rdf:about="https://www.w3.org/ns/ssn/isProducedBy">
        <owl:inverseOf rdf:resource="https://www.w3.org/ns/ssn/produces"/>
        <rdfs:comment>Relation between a producer and a produced entity: for example, between a sensor and the produced output.</rdfs:comment>
        <rdfs:label>is produced by</rdfs:label>
    </owl:ObjectProperty>
    


    <!-- https://www.w3.org/ns/ssn/isPropertyOf -->

    <owl:ObjectProperty rdf:about="https://www.w3.org/ns/ssn/isPropertyOf">
        <rdfs:comment>Relation between a FeatureOfInterest and a Property (a Quality observable by a sensor) of that feature.</rdfs:comment>
        <rdfs:label>is property of</rdfs:label>
    </owl:ObjectProperty>
    


    <!-- https://www.w3.org/ns/ssn/isProxyFor -->

    <rdf:Description rdf:about="https://www.w3.org/ns/ssn/isProxyFor">
        <rdfs:comment>A relation from a Stimulus to the Property that the Stimulus is serving as a proxy for.  For example, the expansion of the quicksilver is a stimulus that serves as a proxy for temperature, or an increase or decrease in the spinning of cups on a wind sensor is serving as a proxy for wind speed.</rdfs:comment>
        <rdfs:label>isProxyFor</rdfs:label>
    </rdf:Description>
    


    <!-- https://www.w3.org/ns/ssn/isValueOf -->

    <owl:ObjectProperty rdf:about="https://www.w3.org/ns/ssn/isValueOf"/>
    


    <!-- https://www.w3.org/ns/ssn/madeObservation -->

    <owl:ObjectProperty rdf:about="https://www.w3.org/ns/ssn/madeObservation">
        <owl:inverseOf rdf:resource="https://www.w3.org/ns/ssn/observedBy"/>
        <rdfs:comment>Relation between a Sensor and Observations it has made.</rdfs:comment>
        <rdfs:label>made observation</rdfs:label>
    </owl:ObjectProperty>
    


    <!-- https://www.w3.org/ns/ssn/observationResult -->

    <rdf:Description rdf:about="https://www.w3.org/ns/ssn/observationResult">
        <dc:source>skos:closeMatch &apos;result&apos; [O&amp;M - ISO/DIS 19156] 
		                    http://portal.opengeospatial.org/files/?artifact_id=41579</dc:source>
        <rdfs:comment>Relation linking an Observation (i.e., a description of the context, the Situation, in which the observatioin was made) and a Result, which contains a value representing the value associated with the observed Property.</rdfs:comment>
        <rdfs:label>observation result</rdfs:label>
    </rdf:Description>
    


    <!-- https://www.w3.org/ns/ssn/observationResultTime -->

    <rdf:Description rdf:about="https://www.w3.org/ns/ssn/observationResultTime">
        <dc:source>http://www.opengeospatial.org/standards/om</dc:source>
        <rdfs:comment>The result time is the time when the procedure associated with the observation act was applied.</rdfs:comment>
        <rdfs:comment>The result time shall describe the time when the result became available, typically when the procedure associated with the observation was completed For some observations this is identical to the phenomenonTime. However, there are important cases where they differ.[O&amp;M]</rdfs:comment>
        <rdfs:label>observation result time</rdfs:label>
    </rdf:Description>
    


    <!-- https://www.w3.org/ns/ssn/observationSamplingTime -->

    <rdf:Description rdf:about="https://www.w3.org/ns/ssn/observationSamplingTime">
        <dc:source>http://www.opengeospatial.org/standards/om</dc:source>
        <rdfs:comment>Rebadged as phenomenon time in [O&amp;M]. The phenomenon time shall describe the time that the result applies to the property of the feature-of-interest. This is often the time of interaction by a sampling procedure or observation procedure with a real-world feature.</rdfs:comment>
        <rdfs:comment>The sampling time is the time that the result applies to the feature-of-interest. This is the time usually required for geospatial analysis of the result.</rdfs:comment>
        <rdfs:label>observation sampling time</rdfs:label>
    </rdf:Description>
    


    <!-- https://www.w3.org/ns/ssn/observedBy -->

    <owl:ObjectProperty rdf:about="https://www.w3.org/ns/ssn/observedBy"/>
    


    <!-- https://www.w3.org/ns/ssn/observedProperty -->

    <rdf:Description rdf:about="https://www.w3.org/ns/ssn/observedProperty">
        <dc:source>skos:exactMatch &apos;observedProperty&apos; [O&amp;M - ISO/DIS 19156] 
		                    http://portal.opengeospatial.org/files/?artifact_id=41579</dc:source>
        <rdfs:comment>Relation linking an Observation to the Property that was observed.  The observedProperty should be a Property (hasProperty) of the FeatureOfInterest (linked by featureOfInterest) of this observation.</rdfs:comment>
        <rdfs:label>observed property</rdfs:label>
    </rdf:Description>
    


    <!-- https://www.w3.org/ns/ssn/observes -->

    <owl:ObjectProperty rdf:about="https://www.w3.org/ns/ssn/observes">
        <rdfs:subPropertyOf rdf:resource="http://www.w3.org/2002/07/owl#topObjectProperty"/>
        <owl:propertyChainAxiom rdf:parseType="Collection">
            <rdf:Description rdf:about="https://www.w3.org/ns/ssn/hasMeasurementCapability"/>
            <rdf:Description rdf:about="https://www.w3.org/ns/ssn/forProperty"/>
        </owl:propertyChainAxiom>
        <owl:propertyChainAxiom rdf:parseType="Collection">
            <rdf:Description rdf:about="https://www.w3.org/ns/ssn/madeObservation"/>
            <rdf:Description rdf:about="https://www.w3.org/ns/ssn/observedProperty"/>
        </owl:propertyChainAxiom>
    </owl:ObjectProperty>
    


    <!-- https://www.w3.org/ns/ssn/ofFeature -->

    <rdf:Description rdf:about="https://www.w3.org/ns/ssn/ofFeature">
        <rdfs:comment>A relation between some aspect of a sensing entity and a feature.  For example, from a sensor to the features it can observe properties of, or from a deployment to the features it was installed to observe.  Also from a measurement capability to the feature the capability is described for.  (Used in conjunction with forProperty).</rdfs:comment>
        <rdfs:label>of feature</rdfs:label>
    </rdf:Description>
    


    <!-- https://www.w3.org/ns/ssn/onPlatform -->

    <owl:ObjectProperty rdf:about="https://www.w3.org/ns/ssn/onPlatform">
        <rdfs:comment>Relation between a System (e.g., a Sensor) and a Platform.  The relation locates the sensor relative to other described entities entities: i.e., the Sensor s1&apos;s location is Platform p1.  More precise locations for sensors in space (relative to other entities, where attached to another entity, or in 3D space) are made using DOLCE&apos;s Regions (SpaceRegion).</rdfs:comment>
        <rdfs:label>on platform</rdfs:label>
    </owl:ObjectProperty>
    


    <!-- https://www.w3.org/ns/ssn/produces -->

    <owl:ObjectProperty rdf:about="https://www.w3.org/ns/ssn/produces">
        <rdfs:subPropertyOf rdf:resource="http://www.w3.org/2002/07/owl#topObjectProperty"/>
        <owl:propertyChainAxiom rdf:parseType="Collection">
            <rdf:Description rdf:about="https://www.w3.org/ns/ssn/madeObservation"/>
            <rdf:Description rdf:about="https://www.w3.org/ns/ssn/observationResult"/>
        </owl:propertyChainAxiom>
        <rdfs:comment>The chain here means that if a sensor made an observation and that observation has a result, then the result is the one produced by the sensor.  Just ensures that the sensor and the resulting observation agree on the result.</rdfs:comment>
    </owl:ObjectProperty>
    


    <!-- https://www.w3.org/ns/ssn/qualityOfObservation -->

    <owl:ObjectProperty rdf:about="https://www.w3.org/ns/ssn/qualityOfObservation">
        <rdfs:subPropertyOf rdf:resource="https://www.w3.org/ns/ssn/hasProperty"/>
        <dc:source>skos:exactMatch &apos;resultQuality&apos; [O&amp;M - ISO/DIS 19156] 
		                    http://portal.opengeospatial.org/files/?artifact_id=41579</dc:source>
        <rdfs:comment>Relation linking an Observation to the adjudged quality of the result.  This is of course complimentary to the MeasurementCapability information recorded for the Sensor that made the Observation.</rdfs:comment>
        <rdfs:label>quality of observation</rdfs:label>
        <rdfs:seeAlso>http://www.w3.org/2005/Incubator/ssn/wiki/SSN_Observation#Observation</rdfs:seeAlso>
    </owl:ObjectProperty>
    


    <!-- https://www.w3.org/ns/ssn/sensingMethodUsed -->

    <rdf:Description rdf:about="https://www.w3.org/ns/ssn/sensingMethodUsed">
        <dc:source>http://www.bipm.org/en/committees/jc/jcgm/wg2.html</dc:source>
        <rdfs:comment>A (measurement) procedure is a detailed description of a measurement according to one or more measurement principles and to a given measurement method, based on a measurement model and including any calculation to obtain a measurement result [VIM 2.6]</rdfs:comment>
        <rdfs:label>sensing method used</rdfs:label>
    </rdf:Description>
    


    <!-- 
    ///////////////////////////////////////////////////////////////////////////////////////
    //
    // Data properties
    //
    ///////////////////////////////////////////////////////////////////////////////////////
     -->

    


    <!-- http://schema.org/value -->

    <rdf:Description rdf:about="http://schema.org/value">
        <rdfs:comment xml:lang="en">The value of the quantitative value or property value node. For QuantitativeValue and MonetaryValue, the recommended type for values is &apos;Number&apos;. For PropertyValue, it can be &apos;Text;&apos;, &apos;Number&apos;, &apos;Boolean&apos;, or &apos;StructuredValue&apos;.</rdfs:comment>
        <rdfs:label xml:lang="en">value</rdfs:label>
    </rdf:Description>
    


    <!-- 
    ///////////////////////////////////////////////////////////////////////////////////////
    //
    // Classes
    //
    ///////////////////////////////////////////////////////////////////////////////////////
     -->

    


    <!-- http://http://www.esonetyellowpages.com/vocab/AcousticDopplerCurrentProfiler -->

    <owl:Class rdf:about="http://http://www.esonetyellowpages.com/vocab/AcousticDopplerCurrentProfiler">
        <rdfs:subClassOf rdf:resource="http://http://www.esonetyellowpages.com/vocab/HydroacousticCurrentMeter"/>
        <rdfs:subClassOf>
            <owl:Restriction>
                <owl:onProperty rdf:resource="https://www.w3.org/ns/ssn/detects"/>
                <owl:allValuesFrom rdf:resource="http://http://www.esonetyellowpages.com/vocab/DopplerEffect"/>
            </owl:Restriction>
        </rdfs:subClassOf>
        <dc:source rdf:datatype="http://www.w3.org/2001/XMLSchema#anyURI">https://en.wikipedia.org/wiki/Acoustic_Doppler_current_profiler</dc:source>
        <rdfs:comment xml:lang="en">An acoustic Doppler current profiler (ADCP) is a hydroacoustic current meter similar to a sonar, attempting to measure water current velocities over a depth range using the Doppler effect of sound waves scattered back from particles within the water column.</rdfs:comment>
        <rdfs:label xml:lang="en">Acoustic Doppler Current Profiler</rdfs:label>
    </owl:Class>
    


    <!-- http://http://www.esonetyellowpages.com/vocab/CurrentMeter -->

    <owl:Class rdf:about="http://http://www.esonetyellowpages.com/vocab/CurrentMeter">
        <rdfs:subClassOf rdf:resource="http://http://www.esonetyellowpages.com/vocab/OceanographicDevice"/>
        <rdfs:subClassOf>
            <owl:Restriction>
                <owl:onProperty rdf:resource="https://www.w3.org/ns/ssn/observes"/>
                <owl:allValuesFrom rdf:resource="http://http://www.esonetyellowpages.com/vocab/FlowVelocity"/>
            </owl:Restriction>
        </rdfs:subClassOf>
        <dc:source rdf:datatype="http://www.w3.org/2001/XMLSchema#anyURI">https://en.wikipedia.org/wiki/Current_meter</dc:source>
        <rdfs:comment xml:lang="en">A current meter is an oceanographic device for flow measurement by mechanical (rotor current meter), tilt (Tilt Current Meter), acoustical (ADCP) or electrical means.</rdfs:comment>
        <rdfs:label xml:lang="en">Current Meter</rdfs:label>
    </owl:Class>
    


    <!-- http://http://www.esonetyellowpages.com/vocab/DopplerEffect -->

    <owl:Class rdf:about="http://http://www.esonetyellowpages.com/vocab/DopplerEffect">
        <rdfs:subClassOf rdf:resource="https://www.w3.org/ns/ssn/Stimulus"/>
        <rdfs:subClassOf>
            <owl:Restriction>
                <owl:onProperty rdf:resource="https://www.w3.org/ns/ssn/isProxyFor"/>
                <owl:allValuesFrom rdf:resource="http://http://www.esonetyellowpages.com/vocab/FlowVelocity"/>
            </owl:Restriction>
        </rdfs:subClassOf>
        <rdfs:comment xml:lang="en">The Doppler effect (or the Doppler shift) is the change in frequency of a wave (or other periodic event) for an observer moving relative to its source.</rdfs:comment>
        <rdfs:label xml:lang="en">Doppler Effect</rdfs:label>
        <rdfs:seeAlso rdf:datatype="http://www.w3.org/2001/XMLSchema#anyURI">https://en.wikipedia.org/wiki/Doppler_effect</rdfs:seeAlso>
    </owl:Class>
    


    <!-- http://http://www.esonetyellowpages.com/vocab/FixedPointOceanObservatory -->

    <owl:Class rdf:about="http://http://www.esonetyellowpages.com/vocab/FixedPointOceanObservatory">
        <rdfs:subClassOf rdf:resource="http://http://www.esonetyellowpages.com/vocab/OceanObservatory"/>
        <rdfs:label xml:lang="en">Fixed-Point Ocean Observatory</rdfs:label>
    </owl:Class>
    


    <!-- http://http://www.esonetyellowpages.com/vocab/FlowVelocity -->

    <owl:Class rdf:about="http://http://www.esonetyellowpages.com/vocab/FlowVelocity">
        <rdfs:subClassOf rdf:resource="http://http://www.esonetyellowpages.com/vocab/Velocity"/>
        <rdfs:subClassOf>
            <owl:Restriction>
                <owl:onProperty rdf:resource="https://www.w3.org/ns/ssn/isPropertyOf"/>
                <owl:someValuesFrom rdf:resource="http://http://www.esonetyellowpages.com/vocab/Fluid"/>
            </owl:Restriction>
        </rdfs:subClassOf>
        <rdfs:label xml:lang="en">Flow Velocity</rdfs:label>
    </owl:Class>
    


    <!-- http://http://www.esonetyellowpages.com/vocab/Fluid -->

    <owl:Class rdf:about="http://http://www.esonetyellowpages.com/vocab/Fluid">
        <rdfs:subClassOf rdf:resource="https://www.w3.org/ns/ssn/FeatureOfInterest"/>
        <rdfs:label xml:lang="en">Fluid</rdfs:label>
    </owl:Class>
    


    <!-- http://http://www.esonetyellowpages.com/vocab/HydroacousticCurrentMeter -->

    <owl:Class rdf:about="http://http://www.esonetyellowpages.com/vocab/HydroacousticCurrentMeter">
        <rdfs:subClassOf rdf:resource="http://http://www.esonetyellowpages.com/vocab/CurrentMeter"/>
        <rdfs:subClassOf>
            <owl:Restriction>
                <owl:onProperty rdf:resource="https://www.w3.org/ns/ssn/detects"/>
                <owl:allValuesFrom rdf:resource="http://http://www.esonetyellowpages.com/vocab/SoundWave"/>
            </owl:Restriction>
        </rdfs:subClassOf>
        <rdfs:label xml:lang="en">Hydroacoustic Current Meter</rdfs:label>
    </owl:Class>
    


    <!-- http://http://www.esonetyellowpages.com/vocab/OceanObservatory -->

    <owl:Class rdf:about="http://http://www.esonetyellowpages.com/vocab/OceanObservatory">
        <rdfs:subClassOf rdf:resource="https://www.w3.org/ns/ssn/Platform"/>
        <rdfs:label xml:lang="en">Ocean Observatory</rdfs:label>
    </owl:Class>
    


    <!-- http://http://www.esonetyellowpages.com/vocab/OceanographicDevice -->

    <owl:Class rdf:about="http://http://www.esonetyellowpages.com/vocab/OceanographicDevice">
        <rdfs:subClassOf rdf:resource="https://www.w3.org/ns/ssn/SensingDevice"/>
        <rdfs:label xml:lang="en">Oceanographic Device</rdfs:label>
    </owl:Class>
    


    <!-- http://http://www.esonetyellowpages.com/vocab/SoundWave -->

    <owl:Class rdf:about="http://http://www.esonetyellowpages.com/vocab/SoundWave">
        <rdfs:subClassOf rdf:resource="https://www.w3.org/ns/ssn/Stimulus"/>
        <rdfs:label xml:lang="en">Sound Wave</rdfs:label>
    </owl:Class>
    


    <!-- http://http://www.esonetyellowpages.com/vocab/Velocity -->

    <owl:Class rdf:about="http://http://www.esonetyellowpages.com/vocab/Velocity">
        <rdfs:subClassOf rdf:resource="https://www.w3.org/ns/ssn/Property"/>
        <rdfs:label xml:lang="en">Velocity</rdfs:label>
    </owl:Class>
    


    <!-- http://http://www.esonetyellowpages.com/vocab/Water -->

    <owl:Class rdf:about="http://http://www.esonetyellowpages.com/vocab/Water">
        <rdfs:subClassOf rdf:resource="http://http://www.esonetyellowpages.com/vocab/Fluid"/>
        <rdfs:label xml:lang="en">Water</rdfs:label>
    </owl:Class>
    


    <!-- http://http://www.esonetyellowpages.com/vocab/WorkhorseQuartermaster150kHzADCP -->

    <owl:Class rdf:about="http://http://www.esonetyellowpages.com/vocab/WorkhorseQuartermaster150kHzADCP">
        <rdfs:subClassOf rdf:resource="http://http://www.esonetyellowpages.com/vocab/AcousticDopplerCurrentProfiler"/>
        <rdfs:subClassOf>
            <owl:Restriction>
                <owl:onProperty rdf:resource="https://www.w3.org/ns/ssn/hasMeasurementCapability"/>
                <owl:hasValue rdf:resource="http://http://www.esonetyellowpages.com/vocab/Workhorse-Quartermaster-150-kHz-ADCP-Frequency"/>
            </owl:Restriction>
        </rdfs:subClassOf>
        <rdfs:subClassOf>
            <owl:Restriction>
                <owl:onProperty rdf:resource="https://www.w3.org/ns/ssn/hasMeasurementCapability"/>
                <owl:hasValue rdf:resource="http://http://www.esonetyellowpages.com/vocab/Workhorse-Quartermaster-150-kHz-ADCP-Max-Profiling-Range"/>
            </owl:Restriction>
        </rdfs:subClassOf>
        <rdfs:comment xml:lang="en">Teledyne RD Instruments Workhorse Quartermaster 150 kHz ADCP</rdfs:comment>
        <rdfs:label xml:lang="en">Workhorse Quartermaster 150 kHz ADCP</rdfs:label>
        <rdfs:seeAlso xml:lang="en">http://www.esonetyellowpages.com/datasheets/datasheet-adcp_whs_150khz_1458583613.pdf</rdfs:seeAlso>
    </owl:Class>
    


    <!-- http://schema.org/QuantitativeValue -->

    <owl:Class rdf:about="http://schema.org/QuantitativeValue">
        <rdfs:subClassOf>
            <owl:Restriction>
                <owl:onProperty rdf:resource="http://schema.org/unitCode"/>
                <owl:someValuesFrom rdf:resource="http://www.w3.org/2002/07/owl#Thing"/>
            </owl:Restriction>
        </rdfs:subClassOf>
        <rdfs:subClassOf>
            <owl:Restriction>
                <owl:onProperty rdf:resource="http://schema.org/value"/>
                <owl:allValuesFrom rdf:resource="http://www.w3.org/2001/XMLSchema#float"/>
            </owl:Restriction>
        </rdfs:subClassOf>
        <rdfs:comment xml:lang="en">A point value or interval for product characteristics and other purposes.</rdfs:comment>
        <rdfs:label xml:lang="en">Quantitative Value</rdfs:label>
    </owl:Class>
    


    <!-- https://www.w3.org/ns/ssn/Accuracy -->

    <owl:Class rdf:about="https://www.w3.org/ns/ssn/Accuracy">
        <rdfs:subClassOf rdf:resource="https://www.w3.org/ns/ssn/MeasurementProperty"/>
        <dc:source>skos:exactMatch &apos;measurement accuracy/accuracy&apos; [VIM 2.13] 
		                    http://www.bipm.org/utils/common/documents/jcgm/JCGM_200_2008.pdf</dc:source>
        <rdfs:comment>The closeness of agreement between the value of an observation and the true value of the observed quality.</rdfs:comment>
        <rdfs:label>Accuracy</rdfs:label>
    </owl:Class>
    


    <!-- https://www.w3.org/ns/ssn/BatteryLifetime -->

    <owl:Class rdf:about="https://www.w3.org/ns/ssn/BatteryLifetime">
        <rdfs:subClassOf rdf:resource="https://www.w3.org/ns/ssn/SurvivalProperty"/>
        <rdfs:comment>Total useful life of a battery.</rdfs:comment>
        <rdfs:label>Battery Lifetime</rdfs:label>
    </owl:Class>
    


    <!-- https://www.w3.org/ns/ssn/Condition -->

    <owl:Class rdf:about="https://www.w3.org/ns/ssn/Condition">
        <rdfs:subClassOf rdf:resource="https://www.w3.org/ns/ssn/Property"/>
        <rdfs:comment>Used to specify ranges for qualities that act as conditions on a system/sensor&apos;s operation.  For example, wind speed of 10-60m/s is expressed as a condition linking a quality, wind speed, a unit of measurement, metres per second, and a set of values, 10-60, and may be used as the condition on a MeasurementProperty, for example, to state that a sensor has a particular accuracy in that condition.</rdfs:comment>
        <rdfs:label>Condition</rdfs:label>
    </owl:Class>
    


    <!-- https://www.w3.org/ns/ssn/Deployment -->

    <owl:Class rdf:about="https://www.w3.org/ns/ssn/Deployment">
        <rdfs:subClassOf rdf:resource="https://www.w3.org/ns/ssn/DeploymentRelatedProcess"/>
        <rdfs:subClassOf>
            <owl:Restriction>
                <owl:onProperty rdf:resource="https://www.w3.org/ns/ssn/deployedOnPlatform"/>
                <owl:allValuesFrom rdf:resource="https://www.w3.org/ns/ssn/Platform"/>
            </owl:Restriction>
        </rdfs:subClassOf>
        <rdfs:subClassOf>
            <owl:Restriction>
                <owl:onProperty rdf:resource="https://www.w3.org/ns/ssn/deployedSystem"/>
                <owl:allValuesFrom rdf:resource="https://www.w3.org/ns/ssn/System"/>
            </owl:Restriction>
        </rdfs:subClassOf>
        <dc:source>skos:closeMatch &apos;Deployment&apos; [MMI Dev]
                                 http://marinemetadata.org/community/teams/ontdevices</dc:source>
        <rdfs:comment>The ongoing Process of Entities (for the purposes of this ontology, mainly sensors) deployed for a particular purpose.  For example, a particular Sensor deployed on a Platform, or a whole network of Sensors deployed for an observation campaign.  The deployment may have sub processes, such as installation, maintenance, addition, and decomissioning and removal.</rdfs:comment>
        <rdfs:label>Deployment</rdfs:label>
    </owl:Class>
    


    <!-- https://www.w3.org/ns/ssn/DeploymentRelatedProcess -->

    <owl:Class rdf:about="https://www.w3.org/ns/ssn/DeploymentRelatedProcess">
        <rdfs:subClassOf>
            <owl:Restriction>
                <owl:onProperty rdf:resource="https://www.w3.org/ns/ssn/deploymentProcessPart"/>
                <owl:allValuesFrom rdf:resource="https://www.w3.org/ns/ssn/DeploymentRelatedProcess"/>
            </owl:Restriction>
        </rdfs:subClassOf>
        <rdfs:comment>Place to group all the various Processes related to Deployment.  For example, as well as Deplyment, installation, maintenance, deployment of further sensors and the like would all be classified under DeploymentRelatedProcess.</rdfs:comment>
        <rdfs:label>Deployment-related Process</rdfs:label>
    </owl:Class>
    


    <!-- https://www.w3.org/ns/ssn/DetectionLimit -->

    <owl:Class rdf:about="https://www.w3.org/ns/ssn/DetectionLimit">
        <rdfs:subClassOf rdf:resource="https://www.w3.org/ns/ssn/MeasurementProperty"/>
        <dc:source>skos:exactMatch &apos;detection limit&apos; [VIM 4.18] 
                                 http://www.bipm.org/utils/common/documents/jcgm/JCGM_200_2008.pdf</dc:source>
        <rdfs:comment>An observed value for which the probability of falsely claiming the absence of a component in a material is Î², given a probability Î± of falsely claiming its presence.</rdfs:comment>
        <rdfs:label>detection limit</rdfs:label>
    </owl:Class>
    


    <!-- https://www.w3.org/ns/ssn/Device -->

    <owl:Class rdf:about="https://www.w3.org/ns/ssn/Device">
        <rdfs:subClassOf rdf:resource="https://www.w3.org/ns/ssn/System"/>
        <rdfs:comment>A device is a physical piece of technology - a system in a box. Devices may of course be built of smaller devices and software components (i.e. systems have components).</rdfs:comment>
        <rdfs:label>Device</rdfs:label>
    </owl:Class>
    


    <!-- https://www.w3.org/ns/ssn/Drift -->

    <owl:Class rdf:about="https://www.w3.org/ns/ssn/Drift">
        <rdfs:subClassOf rdf:resource="https://www.w3.org/ns/ssn/MeasurementProperty"/>
        <dc:source>skos:exactMatch &apos;instrumental drift&apos; [VIM 4.21]
                                  http://www.bipm.org/utils/common/documents/jcgm/JCGM_200_2008.pdf</dc:source>
        <rdfs:comment>A, continuous or incremental, change in the reported values of observations over time for an unchanging quality.</rdfs:comment>
        <rdfs:label>Drift</rdfs:label>
    </owl:Class>
    


    <!-- https://www.w3.org/ns/ssn/FeatureOfInterest -->

    <owl:Class rdf:about="https://www.w3.org/ns/ssn/FeatureOfInterest">
        <rdfs:subClassOf rdf:resource="http://www.w3.org/2002/07/owl#Thing"/>
        <rdfs:subClassOf>
            <owl:Restriction>
                <owl:onProperty rdf:resource="https://www.w3.org/ns/ssn/hasProperty"/>
                <owl:someValuesFrom rdf:resource="https://www.w3.org/ns/ssn/Property"/>
            </owl:Restriction>
        </rdfs:subClassOf>
        <rdfs:subClassOf>
            <owl:Restriction>
                <owl:onProperty rdf:resource="https://www.w3.org/ns/ssn/hasProperty"/>
                <owl:allValuesFrom rdf:resource="https://www.w3.org/ns/ssn/Property"/>
            </owl:Restriction>
        </rdfs:subClassOf>
        <dc:source>skos:exactMatch &apos;feature&apos; [O&amp;M] 
		                    http://www.opengeospatial.org/standards/om</dc:source>
        <rdfs:comment>A feature is an abstraction of real world phenomena (thing, person, event, etc).</rdfs:comment>
        <rdfs:label>Feature of Interest</rdfs:label>
    </owl:Class>
    


    <!-- https://www.w3.org/ns/ssn/MaintenanceSchedule -->

    <owl:Class rdf:about="https://www.w3.org/ns/ssn/MaintenanceSchedule">
        <rdfs:subClassOf rdf:resource="https://www.w3.org/ns/ssn/OperatingProperty"/>
        <rdfs:comment>Schedule of maintenance for a system/sensor in the specified conditions.</rdfs:comment>
        <rdfs:label>Maintenance Schedule</rdfs:label>
    </owl:Class>
    


    <!-- https://www.w3.org/ns/ssn/MeasurementCapability -->

    <owl:Class rdf:about="https://www.w3.org/ns/ssn/MeasurementCapability">
        <rdfs:subClassOf rdf:resource="https://www.w3.org/ns/ssn/Property"/>
        <rdfs:subClassOf>
            <owl:Restriction>
                <owl:onProperty rdf:resource="https://www.w3.org/ns/ssn/forProperty"/>
                <owl:allValuesFrom rdf:resource="https://www.w3.org/ns/ssn/Property"/>
            </owl:Restriction>
        </rdfs:subClassOf>
        <rdfs:subClassOf>
            <owl:Restriction>
                <owl:onProperty rdf:resource="https://www.w3.org/ns/ssn/hasMeasurementProperty"/>
                <owl:allValuesFrom rdf:resource="https://www.w3.org/ns/ssn/MeasurementProperty"/>
            </owl:Restriction>
        </rdfs:subClassOf>
        <rdfs:subClassOf>
            <owl:Restriction>
                <owl:onProperty rdf:resource="https://www.w3.org/ns/ssn/inCondition"/>
                <owl:allValuesFrom rdf:resource="https://www.w3.org/ns/ssn/Condition"/>
            </owl:Restriction>
        </rdfs:subClassOf>
        <dc:source>Similar idea to MeasurementCapability in MMI Device Ontology
                                  http://marinemetadata.org/community/teams/ontdevices

But the the two express the relationship between constraints and multiple measurement properties differently.

The conditions linked to a MeasurementCapability are skos:exactMatch to &apos;influence quantity&apos; [VIM 2.52]
http://www.bipm.org/utils/common/documents/jcgm/JCGM_200_2008.pdf</dc:source>
        <rdfs:comment>Collects together measurement properties (accuracy, range, precision, etc) and the environmental conditions in which those properties hold, representing a specification of a sensor&apos;s capability in those conditions.

The conditions specified here are those that affect the measurement properties, while those in OperatingRange represent the sensor&apos;s standard operating conditions, including conditions that don&apos;t affect the observations.</rdfs:comment>
        <rdfs:label>Measurement Capability</rdfs:label>
    </owl:Class>
    


    <!-- https://www.w3.org/ns/ssn/MeasurementFrequency -->

    <owl:Class rdf:about="https://www.w3.org/ns/ssn/MeasurementFrequency">
        <rdfs:subClassOf rdf:resource="http://schema.org/QuantitativeValue"/>
        <rdfs:subClassOf rdf:resource="https://www.w3.org/ns/ssn/MeasurementProperty"/>
        <rdfs:comment>The smallest possible time between one observation and the next.</rdfs:comment>
        <rdfs:label>MeasurementFrequency</rdfs:label>
    </owl:Class>
    


    <!-- https://www.w3.org/ns/ssn/MeasurementLatency -->

    <owl:Class rdf:about="https://www.w3.org/ns/ssn/MeasurementLatency">
        <rdfs:subClassOf rdf:resource="https://www.w3.org/ns/ssn/MeasurementProperty"/>
        <rdfs:comment>The time between a request for an observation and the sensor producing a result (not including network latency to retrieve the result, just time from request to measurement.).</rdfs:comment>
        <rdfs:label>MeasurementLatency</rdfs:label>
    </owl:Class>
    


    <!-- https://www.w3.org/ns/ssn/MeasurementProperty -->

    <owl:Class rdf:about="https://www.w3.org/ns/ssn/MeasurementProperty">
        <rdfs:subClassOf rdf:resource="https://www.w3.org/ns/ssn/Property"/>
        <rdfs:comment>An identifiable and observable characteristic of a sensor&apos;s observations or ability to make observations.</rdfs:comment>
        <rdfs:label>Measurement Property</rdfs:label>
    </owl:Class>
    


    <!-- https://www.w3.org/ns/ssn/MeasurementRange -->

    <owl:Class rdf:about="https://www.w3.org/ns/ssn/MeasurementRange">
        <rdfs:subClassOf rdf:resource="http://schema.org/QuantitativeValue"/>
        <rdfs:subClassOf rdf:resource="https://www.w3.org/ns/ssn/MeasurementProperty"/>
        <dc:source>skos:exactMatch &apos;measuring interval/measurement range&apos; [VIM 4.7]
                                  http://www.bipm.org/utils/common/documents/jcgm/JCGM_200_2008.pdf</dc:source>
        <rdfs:comment>The set of values that the sensor can return as the result of an observation under the defined conditions with the defined measurement properties.  (If no conditions are specified or the conditions do not specify a range for the observed qualities, the measurement range is to be taken as the condition for the observed qualities.)</rdfs:comment>
        <rdfs:label>Measurement Range</rdfs:label>
    </owl:Class>
    


    <!-- https://www.w3.org/ns/ssn/Observation -->

    <owl:Class rdf:about="https://www.w3.org/ns/ssn/Observation">
        <rdfs:subClassOf>
            <owl:Restriction>
                <owl:onProperty rdf:resource="https://www.w3.org/ns/ssn/fromStimulus"/>
                <owl:someValuesFrom rdf:resource="https://www.w3.org/ns/ssn/Stimulus"/>
            </owl:Restriction>
        </rdfs:subClassOf>
        <rdfs:subClassOf>
            <owl:Restriction>
                <owl:onProperty rdf:resource="https://www.w3.org/ns/ssn/featureOfInterest"/>
                <owl:allValuesFrom rdf:resource="https://www.w3.org/ns/ssn/FeatureOfInterest"/>
            </owl:Restriction>
        </rdfs:subClassOf>
        <rdfs:subClassOf>
            <owl:Restriction>
                <owl:onProperty rdf:resource="https://www.w3.org/ns/ssn/observationResult"/>
                <owl:allValuesFrom rdf:resource="https://www.w3.org/ns/ssn/SensorOutput"/>
            </owl:Restriction>
        </rdfs:subClassOf>
        <rdfs:subClassOf>
            <owl:Restriction>
                <owl:onProperty rdf:resource="https://www.w3.org/ns/ssn/observedBy"/>
                <owl:allValuesFrom rdf:resource="https://www.w3.org/ns/ssn/Sensor"/>
            </owl:Restriction>
        </rdfs:subClassOf>
        <rdfs:subClassOf>
            <owl:Restriction>
                <owl:onProperty rdf:resource="https://www.w3.org/ns/ssn/observedProperty"/>
                <owl:allValuesFrom rdf:resource="https://www.w3.org/ns/ssn/Property"/>
            </owl:Restriction>
        </rdfs:subClassOf>
        <rdfs:subClassOf>
            <owl:Restriction>
                <owl:onProperty rdf:resource="https://www.w3.org/ns/ssn/sensingMethodUsed"/>
                <owl:allValuesFrom rdf:resource="https://www.w3.org/ns/ssn/Sensing"/>
            </owl:Restriction>
        </rdfs:subClassOf>
        <rdfs:subClassOf>
            <owl:Restriction>
                <owl:onProperty rdf:resource="https://www.w3.org/ns/ssn/featureOfInterest"/>
                <owl:qualifiedCardinality rdf:datatype="http://www.w3.org/2001/XMLSchema#nonNegativeInteger">1</owl:qualifiedCardinality>
                <owl:onClass rdf:resource="https://www.w3.org/ns/ssn/FeatureOfInterest"/>
            </owl:Restriction>
        </rdfs:subClassOf>
        <rdfs:subClassOf>
            <owl:Restriction>
                <owl:onProperty rdf:resource="https://www.w3.org/ns/ssn/observedBy"/>
                <owl:qualifiedCardinality rdf:datatype="http://www.w3.org/2001/XMLSchema#nonNegativeInteger">1</owl:qualifiedCardinality>
                <owl:onClass rdf:resource="https://www.w3.org/ns/ssn/Sensor"/>
            </owl:Restriction>
        </rdfs:subClassOf>
        <rdfs:subClassOf>
            <owl:Restriction>
                <owl:onProperty rdf:resource="https://www.w3.org/ns/ssn/observedProperty"/>
                <owl:qualifiedCardinality rdf:datatype="http://www.w3.org/2001/XMLSchema#nonNegativeInteger">1</owl:qualifiedCardinality>
                <owl:onClass rdf:resource="https://www.w3.org/ns/ssn/Property"/>
            </owl:Restriction>
        </rdfs:subClassOf>
        <rdfs:subClassOf>
            <owl:Restriction>
                <owl:onProperty rdf:resource="https://www.w3.org/ns/ssn/sensingMethodUsed"/>
                <owl:qualifiedCardinality rdf:datatype="http://www.w3.org/2001/XMLSchema#nonNegativeInteger">1</owl:qualifiedCardinality>
                <owl:onClass rdf:resource="https://www.w3.org/ns/ssn/Sensing"/>
            </owl:Restriction>
        </rdfs:subClassOf>
        <dc:source>skos:closeMatch &apos;observation&apos; [O&amp;M] 
		                    http://www.opengeospatial.org/standards/om 

Observation in this ontology and O&amp;M are described differently (O&amp;M records an observation as an act/event), but they record the same thing and are essentially interchangeable.  The difference is in the ontological structure of the two, not the data or use.

Observation here records a Situation (the estimation of the value of a Property) and a description of the method that was used (along with the participants), while O&amp;M interprets an Observation as the event itself; there must, however, have been an event that lead to our situation, so both are records of events.  The distinction is between the event itself and the record of what happened in that event.


skos:closeMatch &apos;measurement result&apos; [VIM 2.9] http://www.bipm.org/utils/common/documents/jcgm/JCGM_200_2008.pdf

Measurement result in VIM is the measured value plus any other relevant information, which means that measurement result and observation will often be associated to the same data (a value, a time, a property, etc.).</dc:source>
        <rdfs:comment>An Observation is a Situation in which a Sensing method has been used to estimate or calculate a value of a Property of a FeatureOfInterest.  Links to Sensing and Sensor describe what made the Observation and how; links to Property and Feature detail what was sensed; the result is the output of a Sensor; other metadata details times etc.</rdfs:comment>
        <rdfs:label>Observation</rdfs:label>
    </owl:Class>
    


    <!-- https://www.w3.org/ns/ssn/ObservationValue -->

    <owl:Class rdf:about="https://www.w3.org/ns/ssn/ObservationValue">
        <rdfs:subClassOf>
            <owl:Restriction>
                <owl:onProperty rdf:resource="https://www.w3.org/ns/ssn/isValueOf"/>
                <owl:someValuesFrom rdf:resource="https://www.w3.org/ns/ssn/SensorOutput"/>
            </owl:Restriction>
        </rdfs:subClassOf>
        <dc:source>skos:exactMatch &apos;measured quantity value&apos; [VIM 2.10]
                                  http://www.bipm.org/utils/common/documents/jcgm/JCGM_200_2008.pdf

skos:exactMatch &apos;observed value&apos; [SensorML OGC-0700]
http://www.opengeospatial.org/standards/sensorml 

skos:closeMatch &apos;observation result&apos; [O&amp;M]
http://www.opengeospatial.org/standards/om 

O&amp;M conflates what we have as SensorOutput and ObservationValue into observation result, though the OGC standard does say &quot;result contains a value&quot; and &quot;a result which has a value&quot;, which fits naturally with the model here.</dc:source>
        <rdfs:comment>The value of the result of an Observation.  An Observation has a result which is the output of some sensor, the result is an information object that encodes some value for a Feature.</rdfs:comment>
        <rdfs:label>Observation Value</rdfs:label>
    </owl:Class>
    


    <!-- https://www.w3.org/ns/ssn/OperatingPowerRange -->

    <owl:Class rdf:about="https://www.w3.org/ns/ssn/OperatingPowerRange">
        <rdfs:subClassOf rdf:resource="https://www.w3.org/ns/ssn/OperatingProperty"/>
        <rdfs:comment>Power range in which system/sensor is expected to operate.</rdfs:comment>
        <rdfs:label>Operating Power Range</rdfs:label>
    </owl:Class>
    


    <!-- https://www.w3.org/ns/ssn/OperatingProperty -->

    <owl:Class rdf:about="https://www.w3.org/ns/ssn/OperatingProperty">
        <rdfs:subClassOf rdf:resource="https://www.w3.org/ns/ssn/Property"/>
        <rdfs:comment>An identifiable characteristic of the environmental and other conditions in which the sensor is intended to operate.  May include power ranges, power sources, standard configurations, attachments and the like.</rdfs:comment>
        <rdfs:label>Operating Property</rdfs:label>
    </owl:Class>
    


    <!-- https://www.w3.org/ns/ssn/OperatingRange -->

    <owl:Class rdf:about="https://www.w3.org/ns/ssn/OperatingRange">
        <rdfs:subClassOf rdf:resource="https://www.w3.org/ns/ssn/Property"/>
        <rdfs:subClassOf>
            <owl:Restriction>
                <owl:onProperty rdf:resource="https://www.w3.org/ns/ssn/hasOperatingProperty"/>
                <owl:allValuesFrom rdf:resource="https://www.w3.org/ns/ssn/OperatingProperty"/>
            </owl:Restriction>
        </rdfs:subClassOf>
        <rdfs:subClassOf>
            <owl:Restriction>
                <owl:onProperty rdf:resource="https://www.w3.org/ns/ssn/inCondition"/>
                <owl:allValuesFrom rdf:resource="https://www.w3.org/ns/ssn/Condition"/>
            </owl:Restriction>
        </rdfs:subClassOf>
        <dc:source>skos:broaderMatch &apos;reference operating condition&apos; [VIM 4.11]
                                  http://www.bipm.org/utils/common/documents/jcgm/JCGM_200_2008.pdf

The difference is that here we also allow for qualities that aren&apos;t VIM influence quantities [VIM 2.52] - for example, a quantity that alters the power requirements, but doesn&apos;t affect the measurement properties - conditions specified in MeasurementCapability should be influence quantities.</dc:source>
        <rdfs:comment>The environmental conditions and characteristics of a system/sensor&apos;s normal operating environment.  Can be used to specify for example the standard environmental conditions in which the sensor is expected to operate (a Condition with no OperatingProperty), or how the environmental and other operating properties relate: i.e., that the maintenance schedule or power requirements differ according to the conditions.</rdfs:comment>
        <rdfs:label>Operating Range</rdfs:label>
    </owl:Class>
    


    <!-- https://www.w3.org/ns/ssn/Platform -->

    <owl:Class rdf:about="https://www.w3.org/ns/ssn/Platform">
        <rdfs:subClassOf>
            <owl:Restriction>
                <owl:onProperty rdf:resource="https://www.w3.org/ns/ssn/attachedSystem"/>
                <owl:allValuesFrom rdf:resource="https://www.w3.org/ns/ssn/System"/>
            </owl:Restriction>
        </rdfs:subClassOf>
        <rdfs:subClassOf>
            <owl:Restriction>
                <owl:onProperty rdf:resource="https://www.w3.org/ns/ssn/inDeployment"/>
                <owl:allValuesFrom rdf:resource="https://www.w3.org/ns/ssn/Deployment"/>
            </owl:Restriction>
        </rdfs:subClassOf>
        <dc:source>skos:exactMatch &apos;platform&apos; [SensorML OGC-0700]
                                  http://www.opengeospatial.org/standards/sensorml</dc:source>
        <rdfs:comment>An Entity to which other Entities can be attached - particuarly Sensors and other Platforms.  For example, a post might act as the Platform, a bouy might act as a Platform, or a fish might act as a Platform for an attached sensor.</rdfs:comment>
        <rdfs:label>Platform</rdfs:label>
    </owl:Class>
    


    <!-- https://www.w3.org/ns/ssn/Precision -->

    <owl:Class rdf:about="https://www.w3.org/ns/ssn/Precision">
        <rdfs:subClassOf rdf:resource="https://www.w3.org/ns/ssn/MeasurementProperty"/>
        <dc:source>skos:exactMatch &apos;measurement precision/precision&apos; [VIM 2.15]
                                   http://www.bipm.org/utils/common/documents/jcgm/JCGM_200_2008.pdf</dc:source>
        <rdfs:comment>The closeness of agreement between replicate observations on an unchanged or similar quality value: i.e., a measure of a sensor&apos;s ability to consitently reproduce an observation.</rdfs:comment>
        <rdfs:label>Precision</rdfs:label>
    </owl:Class>
    


    <!-- https://www.w3.org/ns/ssn/Property -->

    <owl:Class rdf:about="https://www.w3.org/ns/ssn/Property">
        <rdfs:subClassOf>
            <owl:Restriction>
                <owl:onProperty rdf:resource="https://www.w3.org/ns/ssn/isPropertyOf"/>
                <owl:someValuesFrom rdf:resource="https://www.w3.org/ns/ssn/FeatureOfInterest"/>
            </owl:Restriction>
        </rdfs:subClassOf>
        <dc:source>skos:exactMatch &apos;property&apos; [O&amp;M] 
		                    http://www.opengeospatial.org/standards/om</dc:source>
        <rdfs:comment>An observable Quality of an Event or Object.  That is, not a quality of an abstract entity as is also allowed by DUL&apos;s Quality, but rather an aspect of an entity that is intrinsic to and cannot exist without the entity and is observable by a sensor.</rdfs:comment>
        <rdfs:label>Property</rdfs:label>
    </owl:Class>
    


    <!-- https://www.w3.org/ns/ssn/Resolution -->

    <owl:Class rdf:about="https://www.w3.org/ns/ssn/Resolution">
        <rdfs:subClassOf rdf:resource="https://www.w3.org/ns/ssn/MeasurementProperty"/>
        <dc:source>skos:exactMatch &apos;resolution&apos; [VIM 4.14]
                                  http://www.bipm.org/utils/common/documents/jcgm/JCGM_200_2008.pdf</dc:source>
        <rdfs:comment>The smallest difference in the value of a quality being observed that would result in perceptably different values of observation results.</rdfs:comment>
        <rdfs:label>Resolution</rdfs:label>
    </owl:Class>
    


    <!-- https://www.w3.org/ns/ssn/ResponseTime -->

    <owl:Class rdf:about="https://www.w3.org/ns/ssn/ResponseTime">
        <rdfs:subClassOf rdf:resource="https://www.w3.org/ns/ssn/MeasurementProperty"/>
        <dc:source>skos:exactMatch &apos;step response time&apos; [VIM 4.23]
                                  http://www.bipm.org/utils/common/documents/jcgm/JCGM_200_2008.pdf</dc:source>
        <rdfs:comment>The time between a (step) change inthe value of an observed quality and a sensor (possibly with specified error) &apos;settling&apos; on an observed value.</rdfs:comment>
        <rdfs:label>Response time</rdfs:label>
    </owl:Class>
    


    <!-- https://www.w3.org/ns/ssn/Selectivity -->

    <owl:Class rdf:about="https://www.w3.org/ns/ssn/Selectivity">
        <rdfs:subClassOf rdf:resource="https://www.w3.org/ns/ssn/MeasurementProperty"/>
        <dc:source>skos:exactMatch &apos;selectivity&apos; [VIM 4.13]
                                 http://www.bipm.org/utils/common/documents/jcgm/JCGM_200_2008.pdf</dc:source>
        <rdfs:comment>Selectivity is a property of a sensor whereby it provides observed values for one or more qualities such that the values of each quality are independent of other qualities in the phenomenon, body, or substance being investigated.</rdfs:comment>
        <rdfs:label>Selectivity</rdfs:label>
    </owl:Class>
    


    <!-- https://www.w3.org/ns/ssn/Sensing -->

    <rdf:Description rdf:about="https://www.w3.org/ns/ssn/Sensing">
        <dc:source>http://www.w3.org/2005/Incubator/sso/</dc:source>
        <rdfs:comment>The description of a process (i.e. describes the temporal and dataflow dependencies and relationships amongst its parts) that results in the estimation, or calculation, of the value of a phenomenon.</rdfs:comment>
        <rdfs:label>Sensing</rdfs:label>
    </rdf:Description>
    


    <!-- https://www.w3.org/ns/ssn/SensingDevice -->

    <owl:Class rdf:about="https://www.w3.org/ns/ssn/SensingDevice">
        <rdfs:subClassOf rdf:resource="https://www.w3.org/ns/ssn/Device"/>
        <rdfs:subClassOf rdf:resource="https://www.w3.org/ns/ssn/Sensor"/>
        <rdfs:comment>A sensing device is a device that implements sensing.</rdfs:comment>
        <rdfs:label>Sensing Device</rdfs:label>
    </owl:Class>
    


    <!-- https://www.w3.org/ns/ssn/Sensitivity -->

    <owl:Class rdf:about="https://www.w3.org/ns/ssn/Sensitivity">
        <rdfs:subClassOf rdf:resource="https://www.w3.org/ns/ssn/MeasurementProperty"/>
        <dc:source>skos:exactMatch &apos;sensitivity&apos; [VIM 4.12]
                                  http://www.bipm.org/utils/common/documents/jcgm/JCGM_200_2008.pdf</dc:source>
        <rdfs:comment>Sensitivity is the quotient of the change in a result of sensor and the corresponding change in a value of a quality being observed.</rdfs:comment>
        <rdfs:label>Sensitivity</rdfs:label>
    </owl:Class>
    


    <!-- https://www.w3.org/ns/ssn/Sensor -->

    <owl:Class rdf:about="https://www.w3.org/ns/ssn/Sensor">
        <rdfs:subClassOf>
            <owl:Restriction>
                <owl:onProperty rdf:resource="https://www.w3.org/ns/ssn/implements"/>
                <owl:someValuesFrom rdf:resource="https://www.w3.org/ns/ssn/Sensing"/>
            </owl:Restriction>
        </rdfs:subClassOf>
        <rdfs:subClassOf>
            <owl:Restriction>
                <owl:onProperty rdf:resource="https://www.w3.org/ns/ssn/detects"/>
                <owl:allValuesFrom rdf:resource="https://www.w3.org/ns/ssn/Stimulus"/>
            </owl:Restriction>
        </rdfs:subClassOf>
        <rdfs:subClassOf>
            <owl:Restriction>
                <owl:onProperty rdf:resource="https://www.w3.org/ns/ssn/hasMeasurementCapability"/>
                <owl:allValuesFrom rdf:resource="https://www.w3.org/ns/ssn/MeasurementCapability"/>
            </owl:Restriction>
        </rdfs:subClassOf>
        <rdfs:subClassOf>
            <owl:Restriction>
                <owl:onProperty rdf:resource="https://www.w3.org/ns/ssn/observes"/>
                <owl:allValuesFrom rdf:resource="https://www.w3.org/ns/ssn/Property"/>
            </owl:Restriction>
        </rdfs:subClassOf>
        <dc:source>skos:exactMatch &apos;sensor&apos; [SensorML OGC-0700]
		                    http://www.opengeospatial.org/standards/sensorml 

                                skos:closeMatch &apos;observation procedure&apos; [O&amp;M] 
                                http://www.opengeospatial.org/standards/om 

O&amp;M allows sensors, methods, instruments, systems, algorithms and process chains as the processUsed of an observation; this ontology allows a similar range of things (any thing that can do sensing), just they are all grouped under the term sensor (which is thus wider than the O&amp;M concept).</dc:source>
        <rdfs:comment>A sensor can do (implements) sensing: that is, a sensor is any entity that can follow a sensing method and thus observe some Property of a FeatureOfInterest.  Sensors may be physical devices, computational methods, a laboratory setup with a person following a method, or any other thing that can follow a Sensing Method to observe a Property.</rdfs:comment>
        <rdfs:label>Sensor</rdfs:label>
    </owl:Class>
    


    <!-- https://www.w3.org/ns/ssn/SensorOutput -->

    <owl:Class rdf:about="https://www.w3.org/ns/ssn/SensorOutput">
        <rdfs:subClassOf>
            <owl:Restriction>
                <owl:onProperty rdf:resource="https://www.w3.org/ns/ssn/hasValue"/>
                <owl:someValuesFrom rdf:resource="https://www.w3.org/ns/ssn/ObservationValue"/>
            </owl:Restriction>
        </rdfs:subClassOf>
        <rdfs:subClassOf>
            <owl:Restriction>
                <owl:onProperty rdf:resource="https://www.w3.org/ns/ssn/isProducedBy"/>
                <owl:someValuesFrom rdf:resource="https://www.w3.org/ns/ssn/Sensor"/>
            </owl:Restriction>
        </rdfs:subClassOf>
        <dc:source>http://www.w3.org/2005/Incubator/ssn/

                                  skos:closeMatch &apos;observation result&apos; [O&amp;M] 
                                  http://www.opengeospatial.org/standards/om 

See comments at ObservationValue.</dc:source>
        <rdfs:comment>A sensor outputs a piece of information (an observed value), the value itself being represented by an ObservationValue.</rdfs:comment>
        <rdfs:label>Sensor Output</rdfs:label>
    </owl:Class>
    


    <!-- https://www.w3.org/ns/ssn/Stimulus -->

    <owl:Class rdf:about="https://www.w3.org/ns/ssn/Stimulus">
        <rdfs:subClassOf>
            <owl:Restriction>
                <owl:onProperty rdf:resource="https://www.w3.org/ns/ssn/isProxyFor"/>
                <owl:allValuesFrom rdf:resource="https://www.w3.org/ns/ssn/Property"/>
            </owl:Restriction>
        </rdfs:subClassOf>
        <dc:source>http://www.w3.org/2005/Incubator/sso/</dc:source>
        <rdfs:comment>An Event in the real world that &apos;triggers&apos; the sensor.  The properties associated to the stimulus may be different to eventual observed property.  It is the event, not the object that triggers the sensor.</rdfs:comment>
        <rdfs:label>Stimulus</rdfs:label>
    </owl:Class>
    


    <!-- https://www.w3.org/ns/ssn/SurvivalProperty -->

    <owl:Class rdf:about="https://www.w3.org/ns/ssn/SurvivalProperty">
        <rdfs:subClassOf rdf:resource="https://www.w3.org/ns/ssn/Property"/>
        <rdfs:comment>An identifiable characteristic that represents the extent of the sensors useful life.  Might include for example total battery life or number of recharges, or, for sensors that are used only a fixed number of times, the number of observations that can be made before the sensing capability is depleted.</rdfs:comment>
        <rdfs:label>Survival Property</rdfs:label>
    </owl:Class>
    


    <!-- https://www.w3.org/ns/ssn/SurvivalRange -->

    <owl:Class rdf:about="https://www.w3.org/ns/ssn/SurvivalRange">
        <rdfs:subClassOf rdf:resource="https://www.w3.org/ns/ssn/Property"/>
        <rdfs:subClassOf>
            <owl:Restriction>
                <owl:onProperty rdf:resource="https://www.w3.org/ns/ssn/hasSurvivalProperty"/>
                <owl:allValuesFrom rdf:resource="https://www.w3.org/ns/ssn/SurvivalProperty"/>
            </owl:Restriction>
        </rdfs:subClassOf>
        <rdfs:subClassOf>
            <owl:Restriction>
                <owl:onProperty rdf:resource="https://www.w3.org/ns/ssn/inCondition"/>
                <owl:allValuesFrom rdf:resource="https://www.w3.org/ns/ssn/Condition"/>
            </owl:Restriction>
        </rdfs:subClassOf>
        <dc:source>skos:narrowerMatch &apos;limiting operating condition&apos; [VIM 4.10]
                                  http://www.bipm.org/utils/common/documents/jcgm/JCGM_200_2008.pdf</dc:source>
        <rdfs:comment>The conditions a sensor can be exposed to without damage: i.e., the sensor continues to operate as defined using MeasurementCapability.  If, however, the SurvivalRange is exceeded, the sensor is &apos;damaged&apos; and MeasurementCapability specifications may no longer hold.</rdfs:comment>
        <rdfs:label>Survival Range</rdfs:label>
    </owl:Class>
    


    <!-- https://www.w3.org/ns/ssn/System -->

    <owl:Class rdf:about="https://www.w3.org/ns/ssn/System">
        <rdfs:subClassOf>
            <owl:Restriction>
                <owl:onProperty rdf:resource="https://www.w3.org/ns/ssn/hasSubSystem"/>
                <owl:someValuesFrom rdf:resource="https://www.w3.org/ns/ssn/System"/>
            </owl:Restriction>
        </rdfs:subClassOf>
        <rdfs:subClassOf>
            <owl:Restriction>
                <owl:onProperty rdf:resource="https://www.w3.org/ns/ssn/hasDeployment"/>
                <owl:allValuesFrom rdf:resource="https://www.w3.org/ns/ssn/Deployment"/>
            </owl:Restriction>
        </rdfs:subClassOf>
        <rdfs:subClassOf>
            <owl:Restriction>
                <owl:onProperty rdf:resource="https://www.w3.org/ns/ssn/hasOperatingRange"/>
                <owl:allValuesFrom rdf:resource="https://www.w3.org/ns/ssn/OperatingRange"/>
            </owl:Restriction>
        </rdfs:subClassOf>
        <rdfs:subClassOf>
            <owl:Restriction>
                <owl:onProperty rdf:resource="https://www.w3.org/ns/ssn/hasSubSystem"/>
                <owl:allValuesFrom rdf:resource="https://www.w3.org/ns/ssn/System"/>
            </owl:Restriction>
        </rdfs:subClassOf>
        <rdfs:subClassOf>
            <owl:Restriction>
                <owl:onProperty rdf:resource="https://www.w3.org/ns/ssn/hasSurvivalRange"/>
                <owl:allValuesFrom rdf:resource="https://www.w3.org/ns/ssn/SurvivalRange"/>
            </owl:Restriction>
        </rdfs:subClassOf>
        <rdfs:subClassOf>
            <owl:Restriction>
                <owl:onProperty rdf:resource="https://www.w3.org/ns/ssn/onPlatform"/>
                <owl:allValuesFrom rdf:resource="https://www.w3.org/ns/ssn/Platform"/>
            </owl:Restriction>
        </rdfs:subClassOf>
        <rdfs:comment>System is a unit of abstraction for pieces of infrastructure (and we largely care that they are) for sensing. A system has components, its subsystems, which are other systems.</rdfs:comment>
        <rdfs:label>System</rdfs:label>
    </owl:Class>
    


    <!-- https://www.w3.org/ns/ssn/SystemLifetime -->

    <owl:Class rdf:about="https://www.w3.org/ns/ssn/SystemLifetime">
        <rdfs:subClassOf rdf:resource="https://www.w3.org/ns/ssn/SurvivalProperty"/>
        <rdfs:comment>Total useful life of a sensor/system (expressed as total life since manufacture, time in use, number of operations, etc.).</rdfs:comment>
        <rdfs:label>System Lifetime</rdfs:label>
    </owl:Class>
    


    <!-- 
    ///////////////////////////////////////////////////////////////////////////////////////
    //
    // Individuals
    //
    ///////////////////////////////////////////////////////////////////////////////////////
     -->

    


    <!-- http://http://www.esonetyellowpages.com/vocab/ANTARES -->

    <owl:NamedIndividual rdf:about="http://http://www.esonetyellowpages.com/vocab/ANTARES">
        <rdf:type rdf:resource="http://http://www.esonetyellowpages.com/vocab/FixedPointOceanObservatory"/>
        <rdf:type rdf:resource="http://http://www.esonetyellowpages.com/vocab/OceanObservatory"/>
        <rdf:type rdf:resource="https://www.w3.org/ns/ssn/Platform"/>
        <dc:source rdf:datatype="http://www.w3.org/2001/XMLSchema#anyURI">http://www.fixo3.eu/observatory/antares/</dc:source>
        <rdfs:comment xml:lang="en">Multidisciplinary, permanent marine observatory providing high-bandwidth real-time data transmission from deep-sea for geosciences and marine environmental sciences. Site is part of the MOOSE network providing real-time data transmission through two deep cabled moorings. These moorings are complemented by stand-alone mooring near the junction box. Physical and biogeochemical parameters recorded by autonomous sensors with regular maintenance. In addition monthly ship occupation for CTD profiles and seawater collection. Cabled extension of the neutrino telescope is offering connectors for direct link to shore in addition to operational seismometer already in place.</rdfs:comment>
        <rdfs:label xml:lang="en">ANTARES</rdfs:label>
    </owl:NamedIndividual>
    


    <!-- http://http://www.esonetyellowpages.com/vocab/Biscay-AGL -->

    <owl:NamedIndividual rdf:about="http://http://www.esonetyellowpages.com/vocab/Biscay-AGL">
        <rdf:type rdf:resource="http://http://www.esonetyellowpages.com/vocab/FixedPointOceanObservatory"/>
        <rdf:type rdf:resource="http://http://www.esonetyellowpages.com/vocab/OceanObservatory"/>
        <rdf:type rdf:resource="https://www.w3.org/ns/ssn/Platform"/>
        <dc:source rdf:datatype="http://www.w3.org/2001/XMLSchema#anyURI">http://www.fixo3.eu/observatory/biscay-agl/</dc:source>
        <dc:title xml:lang="en">Ocean-meteorological buoy Augusto González de Linares</dc:title>
        <rdfs:comment xml:lang="en">Mooring in SE Bay of Biscay it comprises a fully-equipped ODAS buoy transmitting data in real-time plus monthly hydrographical and biogeochemical sampling of water column from research vessel. Buoy obtains core measurements of meteorological, physical, biogeochemical, and ecological parameters with high significance to weather forecasting and climate monitoring. Data immediately provided through IEO web page (hourly).</rdfs:comment>
        <rdfs:label xml:lang="en">Biscay AGL</rdfs:label>
    </owl:NamedIndividual>
    


    <!-- http://http://www.esonetyellowpages.com/vocab/CIS -->

    <owl:NamedIndividual rdf:about="http://http://www.esonetyellowpages.com/vocab/CIS">
        <rdf:type rdf:resource="http://http://www.esonetyellowpages.com/vocab/FixedPointOceanObservatory"/>
        <rdf:type rdf:resource="http://http://www.esonetyellowpages.com/vocab/OceanObservatory"/>
        <rdf:type rdf:resource="https://www.w3.org/ns/ssn/Platform"/>
        <dc:source rdf:datatype="http://www.w3.org/2001/XMLSchema#anyURI">http://www.fixo3.eu/observatory/cis/</dc:source>
        <dc:title xml:lang="en">Central Irminger Sea</dc:title>
        <rdfs:comment xml:lang="en">Multidisciplinary mooring, located in the Central Irminger Sea, Subpolar North Atlantic and part of the FP7 NACLIM project. The site is located in the centre of the Irminger Gyre, characterized by particular deep winter mixed layer depth. The mixed layer deepening is promoted through the combination of the cyclonic circulation of the Irminger gyre and strong surface buoyancy forcing in winter. Focus of the interdisciplinary research is on the biogeochemical cycling in a potential deep water formtion area. The physical background field (Temperature, Salinity, Currents) of the upper 1500m is surveyed with a number of sensors. Moreover, biogeochemical sensors (O2, Chl-a, zooplankton) is measured in mixed layer. The site area is shared with the LOCO mooring established by the NIOZ in 2002. The sampling and logistics of the moorings is coordinated with the NACLIM project. In Septmber 2014 the CIS observatory was moved little south and the original position is now occupied by the 4 mooring construction as part of the US OOI initiative. With this configuration one observatory (OOI) is located at the center of the gyre, while CIS and LOCO are where typically the strongest buoyancy focring is found (related to the Greenland Tip Jet).</rdfs:comment>
        <rdfs:label xml:lang="en">CIS</rdfs:label>
    </owl:NamedIndividual>
    


    <!-- http://http://www.esonetyellowpages.com/vocab/CVOO -->

    <owl:NamedIndividual rdf:about="http://http://www.esonetyellowpages.com/vocab/CVOO">
        <rdf:type rdf:resource="http://http://www.esonetyellowpages.com/vocab/FixedPointOceanObservatory"/>
        <rdf:type rdf:resource="http://http://www.esonetyellowpages.com/vocab/OceanObservatory"/>
        <rdf:type rdf:resource="https://www.w3.org/ns/ssn/Platform"/>
        <dc:source rdf:datatype="http://www.w3.org/2001/XMLSchema#anyURI">http://www.fixo3.eu/observatory/cvoo/</dc:source>
        <dc:title xml:lang="en">Cape Verde Ocean Observatory</dc:title>
        <rdfs:comment xml:lang="en">This observatory is composed of a mooring and a small vessel maintaining the time-series continuity at Tropical Eastern North Atlantic.</rdfs:comment>
        <rdfs:label xml:lang="en">CVOO</rdfs:label>
    </owl:NamedIndividual>
    


    <!-- http://http://www.esonetyellowpages.com/vocab/DELOS-A -->

    <owl:NamedIndividual rdf:about="http://http://www.esonetyellowpages.com/vocab/DELOS-A">
        <rdf:type rdf:resource="http://http://www.esonetyellowpages.com/vocab/FixedPointOceanObservatory"/>
        <rdf:type rdf:resource="http://http://www.esonetyellowpages.com/vocab/OceanObservatory"/>
        <rdf:type rdf:resource="https://www.w3.org/ns/ssn/Platform"/>
        <dc:source rdf:datatype="http://www.w3.org/2001/XMLSchema#anyURI">http://www.fixo3.eu/observatory/delos-a/</dc:source>
        <dc:title xml:lang="en">Deep-ocean Environmental Long-term Observatory System</dc:title>
        <rdfs:comment xml:lang="en">The DELOS (Deep-ocean Environmental Long-term Observatory System) system comprises two environmental monitoring platforms: DELOS A located in the near field (within 50 m of a sea floor well); and DELOS B located in the far field (~16 km from sea floor infrastructure). DELOS A located on flat (&lt;1° slope), finely sedimented sea floor within petroleum lease Block 18 in a mid- slope area off Angola between the deep-sea fans of the Congo and Kwanza rivers.  The platform hosts a camera module, oceanographic module and acoustic module, each with multiple instruments.</rdfs:comment>
        <rdfs:label xml:lang="en">DELOS A</rdfs:label>
    </owl:NamedIndividual>
    


    <!-- http://http://www.esonetyellowpages.com/vocab/DELOS-B -->

    <owl:NamedIndividual rdf:about="http://http://www.esonetyellowpages.com/vocab/DELOS-B">
        <rdf:type rdf:resource="http://http://www.esonetyellowpages.com/vocab/FixedPointOceanObservatory"/>
        <rdf:type rdf:resource="http://http://www.esonetyellowpages.com/vocab/OceanObservatory"/>
        <rdf:type rdf:resource="https://www.w3.org/ns/ssn/Platform"/>
        <dc:source rdf:datatype="http://www.w3.org/2001/XMLSchema#anyURI">http://www.fixo3.eu/observatory/delos-b/</dc:source>
        <dc:title xml:lang="en">Deep-ocean Environmental Long-term Observatory System</dc:title>
        <rdfs:comment xml:lang="en">The DELOS (Deep-ocean Environmental Long-term Observatory System) system comprises two environmental monitoring platforms: DELOS A located in the near field (within 50 m of a sea floor well); and DELOS B located in the far field (~16 km from sea floor infrastructure). DELOS B located on flat (&lt;1° slope), finely sedimented sea floor within petroleum lease Block 18 in a mid- slope area off Angola, between the deep-sea fans of the Congo and Kwanza rivers.  The platform hosts a camera module, oceanographic module and acoustic module, each with multiple instruments, plus a sediment trap module.</rdfs:comment>
        <rdfs:label xml:lang="en">DELOS B</rdfs:label>
    </owl:NamedIndividual>
    


    <!-- http://http://www.esonetyellowpages.com/vocab/DYFAMED -->

    <owl:NamedIndividual rdf:about="http://http://www.esonetyellowpages.com/vocab/DYFAMED">
        <rdf:type rdf:resource="http://http://www.esonetyellowpages.com/vocab/FixedPointOceanObservatory"/>
        <rdf:type rdf:resource="http://http://www.esonetyellowpages.com/vocab/OceanObservatory"/>
        <rdf:type rdf:resource="https://www.w3.org/ns/ssn/Platform"/>
        <dc:source rdf:datatype="http://www.w3.org/2001/XMLSchema#anyURI">http://www.fixo3.eu/observatory/dyfamed/</dc:source>
        <dc:title xml:lang="en">Dynamique des Flux Atmospheriques en MEDiterranee</dc:title>
        <rdfs:comment xml:lang="en">Multidisciplinary site within MOOSE network (Ligurian Sea), in passage between eastern and western Med Sea. Strong influence of atmospheric deposition influencing productivity and particle export monitored by atmospheric survey (Cap Ferrat) and two permanent sediment traps. Physical parameters recorded from surface to deep waters through monthly visits and permanent deep mooring. Biogeochemical parameters obtained monthly during ship visits. The site is also a way point of gliders and used for cross- validation of bio-parameters (nitrate, oxygen).</rdfs:comment>
        <rdfs:label xml:lang="en">DYFAMED</rdfs:label>
    </owl:NamedIndividual>
    


    <!-- http://http://www.esonetyellowpages.com/vocab/E1-M3A -->

    <owl:NamedIndividual rdf:about="http://http://www.esonetyellowpages.com/vocab/E1-M3A">
        <rdf:type rdf:resource="http://http://www.esonetyellowpages.com/vocab/FixedPointOceanObservatory"/>
        <rdf:type rdf:resource="http://http://www.esonetyellowpages.com/vocab/OceanObservatory"/>
        <rdf:type rdf:resource="https://www.w3.org/ns/ssn/Platform"/>
        <dc:source rdf:datatype="http://www.w3.org/2001/XMLSchema#anyURI">http://www.fixo3.eu/observatory/e1-m3a/</dc:source>
        <dc:title xml:lang="en">POSEIDON E1-M3A</dc:title>
        <rdfs:comment xml:lang="en">Multidisciplinary mooring located at the eastern Mediterranean off shore Crete island, an area of open sea conditions, characterized as extremely oligotrophic where dense waters with intermediate and deep characteristics are formed.</rdfs:comment>
        <rdfs:label xml:lang="en">E1-M3A</rdfs:label>
    </owl:NamedIndividual>
    


    <!-- http://http://www.esonetyellowpages.com/vocab/E2-M3A -->

    <owl:NamedIndividual rdf:about="http://http://www.esonetyellowpages.com/vocab/E2-M3A">
        <rdf:type rdf:resource="http://http://www.esonetyellowpages.com/vocab/FixedPointOceanObservatory"/>
        <rdf:type rdf:resource="http://http://www.esonetyellowpages.com/vocab/OceanObservatory"/>
        <rdf:type rdf:resource="https://www.w3.org/ns/ssn/Platform"/>
        <ssn:attachedSystem rdf:resource="http://http://www.esonetyellowpages.com/vocab/E2-M3A-ADCP-WHS-150Khz"/>
        <dc:title xml:lang="en">Southern Adriatic Interdisciplinary Laboratory for Ocean Research</dc:title>
        <rdfs:comment xml:lang="en">Deep-sea, continuous monitoring station: it provides the longest oceanographic time series in the South Adriatic Pit (Eastern Mediterranean Sea). The observatory is composed by two moorings (surface buoy and sub-surface mooring line) and designed to monitor physical and biogeochemical processes in the water column from the surface down to the bottom (approximately 1220m).  The E2-M3A surface buoy collects air/sea meteorological and physical measurements in the surface layer (2m depth). The secondary deep mooring instead, is equipped with current meters (RDI-ADCP and Seaguard-RCM), CTD’s with Dissolved Oxygen and optical sensors. New biochemical sensors (CO2 and pH) were deployed during the first year of the FiXO3 project to enhance the payload of the site.</rdfs:comment>
        <rdfs:label xml:lang="en">E2-M3A</rdfs:label>
        <rdfs:seeAlso rdf:datatype="http://www.w3.org/2001/XMLSchema#anyURI">http://www.fixo3.eu/observatory/e2-m3a/</rdfs:seeAlso>
    </owl:NamedIndividual>
    


    <!-- http://http://www.esonetyellowpages.com/vocab/E2-M3A-ADCP-WHS-150Khz -->

    <owl:NamedIndividual rdf:about="http://http://www.esonetyellowpages.com/vocab/E2-M3A-ADCP-WHS-150Khz">
        <rdf:type rdf:resource="http://http://www.esonetyellowpages.com/vocab/AcousticDopplerCurrentProfiler"/>
        <rdf:type rdf:resource="http://http://www.esonetyellowpages.com/vocab/CurrentMeter"/>
        <rdf:type rdf:resource="http://http://www.esonetyellowpages.com/vocab/HydroacousticCurrentMeter"/>
        <rdf:type rdf:resource="http://http://www.esonetyellowpages.com/vocab/OceanographicDevice"/>
        <rdf:type rdf:resource="http://http://www.esonetyellowpages.com/vocab/WorkhorseQuartermaster150kHzADCP"/>
        <rdf:type rdf:resource="https://www.w3.org/ns/ssn/Device"/>
        <rdf:type rdf:resource="https://www.w3.org/ns/ssn/SensingDevice"/>
        <rdf:type rdf:resource="https://www.w3.org/ns/ssn/Sensor"/>
        <rdf:type rdf:resource="https://www.w3.org/ns/ssn/System"/>
        <ssn:hasMeasurementCapability rdf:resource="http://http://www.esonetyellowpages.com/vocab/Workhorse-Quartermaster-150-kHz-ADCP-Frequency"/>
        <ssn:hasMeasurementCapability rdf:resource="http://http://www.esonetyellowpages.com/vocab/Workhorse-Quartermaster-150-kHz-ADCP-Max-Profiling-Range"/>
        <ssn:hasProperty rdf:resource="http://http://www.esonetyellowpages.com/vocab/Workhorse-Quartermaster-150-kHz-ADCP-Frequency"/>
        <ssn:hasProperty rdf:resource="http://http://www.esonetyellowpages.com/vocab/Workhorse-Quartermaster-150-kHz-ADCP-Max-Profiling-Range"/>
        <ssn:onPlatform rdf:resource="http://http://www.esonetyellowpages.com/vocab/E2-M3A"/>
        <rdfs:label xml:lang="en">The Workhorse Quartermaster 150 kHz ADCP on E2-M3A</rdfs:label>
    </owl:NamedIndividual>
    


    <!-- http://http://www.esonetyellowpages.com/vocab/ESTOC -->

    <owl:NamedIndividual rdf:about="http://http://www.esonetyellowpages.com/vocab/ESTOC">
        <rdf:type rdf:resource="http://http://www.esonetyellowpages.com/vocab/FixedPointOceanObservatory"/>
        <rdf:type rdf:resource="http://http://www.esonetyellowpages.com/vocab/OceanObservatory"/>
        <rdf:type rdf:resource="https://www.w3.org/ns/ssn/Platform"/>
        <dc:source rdf:datatype="http://www.w3.org/2001/XMLSchema#anyURI">http://www.fixo3.eu/observatory/estoc/</dc:source>
        <dc:title xml:lang="en">European Station for Time series in the Ocean Canary Islands</dc:title>
        <rdfs:comment xml:lang="en">Multidisciplinary mooring, located in the Central Eastern Atlantic, open ocean site with over 15 years of continuous surface and mid-water meteorological, physical and biogeochemical monitoring.</rdfs:comment>
        <rdfs:label xml:lang="en">ESTOC</rdfs:label>
    </owl:NamedIndividual>
    


    <!-- http://http://www.esonetyellowpages.com/vocab/FILCHNER-RONNE -->

    <owl:NamedIndividual rdf:about="http://http://www.esonetyellowpages.com/vocab/FILCHNER-RONNE">
        <rdf:type rdf:resource="http://http://www.esonetyellowpages.com/vocab/FixedPointOceanObservatory"/>
        <rdf:type rdf:resource="http://http://www.esonetyellowpages.com/vocab/OceanObservatory"/>
        <rdf:type rdf:resource="https://www.w3.org/ns/ssn/Platform"/>
        <dc:source rdf:datatype="http://www.w3.org/2001/XMLSchema#anyURI">http://www.fixo3.eu/observatory/filchner-ronne/</dc:source>
        <dc:title xml:lang="en">S2 observatory Filchner Ronne</dc:title>
        <rdfs:comment xml:lang="en">The S2 Observatory for long term monitoring of Ice Shelf Water (ISW) Overflow situated at the Filchner sill in the southern Weddell Sea was established in 1977 and continues to deliver the longest existing marine time series from Antarctica. The position for the observatory S2 proved to be a key site for monitoring the ISW overflow produced beneath the huge Filchner Ronne Ice Shelf and is selected to be a part of the global net of monitoring sites under CLIVAR (www.clivar.org) and OceanSITES (www.oceansites.org). Time series of current speed and direction, temperature and salinity exist back to 1977.  Continuous observation of dissolved oxygen started in 2009.</rdfs:comment>
        <rdfs:label xml:lang="en">FILCHNER RONNE</rdfs:label>
    </owl:NamedIndividual>
    


    <!-- http://http://www.esonetyellowpages.com/vocab/FRAM -->

    <owl:NamedIndividual rdf:about="http://http://www.esonetyellowpages.com/vocab/FRAM">
        <rdf:type rdf:resource="http://http://www.esonetyellowpages.com/vocab/FixedPointOceanObservatory"/>
        <rdf:type rdf:resource="http://http://www.esonetyellowpages.com/vocab/OceanObservatory"/>
        <rdf:type rdf:resource="https://www.w3.org/ns/ssn/Platform"/>
        <dc:source rdf:datatype="http://www.w3.org/2001/XMLSchema#anyURI">http://www.fixo3.eu/observatory/fram/</dc:source>
        <dc:title xml:lang="en">Frontiers in Arctic Marine Monitoring</dc:title>
        <rdfs:comment xml:lang="en">Array of moorings and permanent sampling sites across the Fram Strait. Installed to capture the exchange of Atlantic and Arctic waters, and to study the temporal development of an Arctic marine ecosystem. Enables year-round multidisciplinary long-term observations, partially with near real-time data access.</rdfs:comment>
        <rdfs:label xml:lang="en">FRAM</rdfs:label>
    </owl:NamedIndividual>
    


    <!-- http://http://www.esonetyellowpages.com/vocab/LION -->

    <owl:NamedIndividual rdf:about="http://http://www.esonetyellowpages.com/vocab/LION">
        <rdf:type rdf:resource="http://http://www.esonetyellowpages.com/vocab/FixedPointOceanObservatory"/>
        <rdf:type rdf:resource="http://http://www.esonetyellowpages.com/vocab/OceanObservatory"/>
        <rdf:type rdf:resource="https://www.w3.org/ns/ssn/Platform"/>
        <dc:source rdf:datatype="http://www.w3.org/2001/XMLSchema#anyURI">http://www.fixo3.eu/observatory/lion/</dc:source>
        <dc:title xml:lang="en">LION</dc:title>
        <rdfs:comment xml:lang="en">Deep-sea mooring located in the convection cell in the centre of the Gulf of Lion which aims to observe the winter convection affecting the north-western Mediterranean Sea water circulation and deep-sea ecosystem (physical data). The mooring is deployed near the ODAS meteorological surface buoy (Gulf of Lion) and integrated in the MOOSE network.</rdfs:comment>
        <rdfs:label xml:lang="en">LION</rdfs:label>
    </owl:NamedIndividual>
    


    <!-- http://http://www.esonetyellowpages.com/vocab/MOMAR -->

    <owl:NamedIndividual rdf:about="http://http://www.esonetyellowpages.com/vocab/MOMAR">
        <rdf:type rdf:resource="http://http://www.esonetyellowpages.com/vocab/FixedPointOceanObservatory"/>
        <rdf:type rdf:resource="http://http://www.esonetyellowpages.com/vocab/OceanObservatory"/>
        <rdf:type rdf:resource="https://www.w3.org/ns/ssn/Platform"/>
        <dc:source rdf:datatype="http://www.w3.org/2001/XMLSchema#anyURI">http://www.fixo3.eu/observatory/momar/</dc:source>
        <dc:title xml:lang="en">MoMAR EMSO Azores</dc:title>
        <rdfs:comment xml:lang="en">Multidisciplinary (fauna, fluid chemistry, seismicity and ground deformation) situated at the mid-Atlantic (hydrothermal vent field Lucky Strike); near real time communication through acoustic link, buoy and satellite. EMSO observatory node, in operation since 2010, comprises an oceanographic mooring and nested arrays of seismometers, pressure probes, temperature probes and chemical sensors in vent fluids, as well as a camera and colonization devices for faunal and microfaunal studies. Satellite transmission of a data subset, accessible on an EMSO-related server. Yearly maintenance cruises scheduled till 2015. Upgrades of system planned for 2014 with several new connection nodes  accessible to FiXO3 collaborations.</rdfs:comment>
        <rdfs:label xml:lang="en">MOMAR</rdfs:label>
    </owl:NamedIndividual>
    


    <!-- http://http://www.esonetyellowpages.com/vocab/NEMO-SN1 -->

    <owl:NamedIndividual rdf:about="http://http://www.esonetyellowpages.com/vocab/NEMO-SN1">
        <rdf:type rdf:resource="http://http://www.esonetyellowpages.com/vocab/FixedPointOceanObservatory"/>
        <rdf:type rdf:resource="http://http://www.esonetyellowpages.com/vocab/OceanObservatory"/>
        <rdf:type rdf:resource="https://www.w3.org/ns/ssn/Platform"/>
        <dc:source rdf:datatype="http://www.w3.org/2001/XMLSchema#anyURI">http://www.fixo3.eu/observatory/nemo-sn1/</dc:source>
        <dc:title xml:lang="en">NEMO-SN1</dc:title>
        <rdfs:comment xml:lang="en">Multidisciplinary (geophysics, oceanography, bio-acoustics) observatory, located in Western Ionian See, offshore Catania (Sicily), deep-sea real-time multi-parameter observatory is currently being re-deployed after refurbishment and installations of new electronics.</rdfs:comment>
        <rdfs:label xml:lang="en">NEMO-SN1</rdfs:label>
    </owl:NamedIndividual>
    


    <!-- http://http://www.esonetyellowpages.com/vocab/NOG -->

    <owl:NamedIndividual rdf:about="http://http://www.esonetyellowpages.com/vocab/NOG">
        <rdf:type rdf:resource="http://http://www.esonetyellowpages.com/vocab/FixedPointOceanObservatory"/>
        <rdf:type rdf:resource="http://http://www.esonetyellowpages.com/vocab/OceanObservatory"/>
        <rdf:type rdf:resource="https://www.w3.org/ns/ssn/Platform"/>
        <dc:source rdf:datatype="http://www.w3.org/2001/XMLSchema#anyURI">http://www.fixo3.eu/observatory/nog/</dc:source>
        <dc:title xml:lang="en">Northern Oligotrophic Gyre</dc:title>
        <rdfs:comment xml:lang="en">Currently comprising a sediment trap mooring with current sensors it is situated in the middle of the least productive gyre in the North Atlantic but one which is influenced to a degree by dust supply from the Sahara desert.</rdfs:comment>
        <rdfs:label xml:lang="en">NOG</rdfs:label>
    </owl:NamedIndividual>
    


    <!-- http://http://www.esonetyellowpages.com/vocab/OBSEA -->

    <owl:NamedIndividual rdf:about="http://http://www.esonetyellowpages.com/vocab/OBSEA">
        <rdf:type rdf:resource="http://http://www.esonetyellowpages.com/vocab/FixedPointOceanObservatory"/>
        <rdf:type rdf:resource="http://http://www.esonetyellowpages.com/vocab/OceanObservatory"/>
        <rdf:type rdf:resource="https://www.w3.org/ns/ssn/Platform"/>
        <dc:source rdf:datatype="http://www.w3.org/2001/XMLSchema#anyURI">http://www.fixo3.eu/observatory/obsea/</dc:source>
        <dc:title xml:lang="en">Expandable Seafloor Observatory</dc:title>
        <rdfs:comment xml:lang="en">The main objective of this site located at Western Mediterranean is to be a test bed for the development of oceanographic instrumentation while being a shallow-water observatory providing real time data and database with historical values.</rdfs:comment>
        <rdfs:label xml:lang="en">OBSEA</rdfs:label>
    </owl:NamedIndividual>
    


    <!-- http://http://www.esonetyellowpages.com/vocab/PAP -->

    <owl:NamedIndividual rdf:about="http://http://www.esonetyellowpages.com/vocab/PAP">
        <rdf:type rdf:resource="http://http://www.esonetyellowpages.com/vocab/FixedPointOceanObservatory"/>
        <rdf:type rdf:resource="http://http://www.esonetyellowpages.com/vocab/OceanObservatory"/>
        <rdf:type rdf:resource="https://www.w3.org/ns/ssn/Platform"/>
        <dc:source rdf:datatype="http://www.w3.org/2001/XMLSchema#anyURI">http://www.fixo3.eu/observatory/pap/</dc:source>
        <dc:title xml:lang="en">Porcupine Abyssal Plain Observatory</dc:title>
        <rdfs:comment xml:lang="en">Array of moorings covering the entire water column and benthos with associated repeat ship occupations for process studies and collections not possible autonomously (eg benthic megafauna) Longest running multidisciplinary North Atlantic open ocean sustained observatory delivering atmospheric and physical and biogeochemical ocean datasets in near real-time.</rdfs:comment>
        <rdfs:label xml:lang="en">PAP</rdfs:label>
    </owl:NamedIndividual>
    


    <!-- http://http://www.esonetyellowpages.com/vocab/PYLOS -->

    <owl:NamedIndividual rdf:about="http://http://www.esonetyellowpages.com/vocab/PYLOS">
        <rdf:type rdf:resource="http://http://www.esonetyellowpages.com/vocab/FixedPointOceanObservatory"/>
        <rdf:type rdf:resource="http://http://www.esonetyellowpages.com/vocab/OceanObservatory"/>
        <rdf:type rdf:resource="https://www.w3.org/ns/ssn/Platform"/>
        <dc:source rdf:datatype="http://www.w3.org/2001/XMLSchema#anyURI">http://www.fixo3.eu/observatory/pylos/</dc:source>
        <dc:title xml:lang="en">Pylos Observatory</dc:title>
        <rdfs:comment xml:lang="en">Multidisciplinary observatory mooring located in the cross road of Adriatic and Eastern Mediterranean basins. Very geologically active area with lots of earthquakes and landslides as well as a potential source of Tsunamis that might affect the Eastern Mediterranean Sea.</rdfs:comment>
        <rdfs:label xml:lang="en">PYLOS</rdfs:label>
    </owl:NamedIndividual>
    


    <!-- http://http://www.esonetyellowpages.com/vocab/SOG -->

    <owl:NamedIndividual rdf:about="http://http://www.esonetyellowpages.com/vocab/SOG">
        <rdf:type rdf:resource="http://http://www.esonetyellowpages.com/vocab/FixedPointOceanObservatory"/>
        <rdf:type rdf:resource="http://http://www.esonetyellowpages.com/vocab/OceanObservatory"/>
        <rdf:type rdf:resource="https://www.w3.org/ns/ssn/Platform"/>
        <dc:source rdf:datatype="http://www.w3.org/2001/XMLSchema#anyURI">http://www.fixo3.eu/observatory/sog/</dc:source>
        <dc:title xml:lang="en">Southern Oligotrophic Gyre</dc:title>
        <rdfs:comment xml:lang="en">Currently comprising a sediment trap mooring with current sensors it is situated in the middle of the least productive gyre in the South Atlantic but in contrast to NOG, an observatory in the North Atlantic oligotrophic gyre, it is not influenced by dust supply.</rdfs:comment>
        <rdfs:label xml:lang="en">SOG</rdfs:label>
    </owl:NamedIndividual>
    


    <!-- http://http://www.esonetyellowpages.com/vocab/SOR -->

    <owl:NamedIndividual rdf:about="http://http://www.esonetyellowpages.com/vocab/SOR">
        <rdf:type rdf:resource="http://http://www.esonetyellowpages.com/vocab/FixedPointOceanObservatory"/>
        <rdf:type rdf:resource="http://http://www.esonetyellowpages.com/vocab/OceanObservatory"/>
        <rdf:type rdf:resource="https://www.w3.org/ns/ssn/Platform"/>
        <dc:source rdf:datatype="http://www.w3.org/2001/XMLSchema#anyURI">http://www.fixo3.eu/observatory/sor/</dc:source>
        <rdfs:comment xml:lang="en">Single location mooring situated on the Mid-Atlantic Ridge south of Svalbard. A component of NOON (Norwegian Ocean Observatory Network) planned as demo mission in 2012 and then as sustained observatory in 2016.</rdfs:comment>
        <rdfs:label xml:lang="en">SOR</rdfs:label>
    </owl:NamedIndividual>
    


    <!-- http://http://www.esonetyellowpages.com/vocab/STATION-M -->

    <owl:NamedIndividual rdf:about="http://http://www.esonetyellowpages.com/vocab/STATION-M">
        <rdf:type rdf:resource="http://http://www.esonetyellowpages.com/vocab/FixedPointOceanObservatory"/>
        <rdf:type rdf:resource="http://http://www.esonetyellowpages.com/vocab/OceanObservatory"/>
        <rdf:type rdf:resource="https://www.w3.org/ns/ssn/Platform"/>
        <dc:source rdf:datatype="http://www.w3.org/2001/XMLSchema#anyURI">http://www.fixo3.eu/observatory/station-m/</dc:source>
        <dc:title xml:lang="en">Station M</dc:title>
        <rdfs:comment xml:lang="en">Ocean Weather Station M (OWS M) has been an ocean weather station since 1948. At present there is a mooring and a surface buoy at the site, which measures hydrography, O2, chlorophyll and carbon parameters. Located in Norwegian Sea with real-time and delayed mode capabilities. The site present the longest existing homogeneous time series from deep ocean. The facility presented here is the mooring situated betveen 150 and 2000 m.

</rdfs:comment>
        <rdfs:label xml:lang="en">STATION M</rdfs:label>
    </owl:NamedIndividual>
    


    <!-- http://http://www.esonetyellowpages.com/vocab/W1-M3A -->

    <owl:NamedIndividual rdf:about="http://http://www.esonetyellowpages.com/vocab/W1-M3A">
        <rdf:type rdf:resource="http://http://www.esonetyellowpages.com/vocab/FixedPointOceanObservatory"/>
        <rdf:type rdf:resource="http://http://www.esonetyellowpages.com/vocab/OceanObservatory"/>
        <rdf:type rdf:resource="https://www.w3.org/ns/ssn/Platform"/>
        <dc:source rdf:datatype="http://www.w3.org/2001/XMLSchema#anyURI">http://www.fixo3.eu/observatory/w1-m3a/</dc:source>
        <rdfs:comment xml:lang="en">A single multidisciplinary observatory mooring located in the Ligurian Sea with real-time and delayed mode capability. The W1-M3A observing system is composed by a large spare buoy and a sub-surface mooring periodically deployed close to the main buoy depending on specific research needs. The W1-M3A large spar buoy specifically designed for air-sea interaction studies and the collection of meteorological data even in rough sea. Stability is the basic feature of this type of buoy with respect to the other more classical approach based on discus-shaped buoys. The buoy was specifically designed as a stable measuring platform since its total mass, the unity buoyancy at the sea level, and presence of a damping disk allow for negligible sensitivity of sea heave and height.</rdfs:comment>
        <rdfs:label xml:lang="en">W1-M3A</rdfs:label>
    </owl:NamedIndividual>
    


    <!-- http://http://www.esonetyellowpages.com/vocab/Workhorse-Quartermaster-150-kHz-ADCP-Frequency -->

    <owl:NamedIndividual rdf:about="http://http://www.esonetyellowpages.com/vocab/Workhorse-Quartermaster-150-kHz-ADCP-Frequency">
        <rdf:type rdf:resource="https://www.w3.org/ns/ssn/MeasurementCapability"/>
        <rdf:type rdf:resource="https://www.w3.org/ns/ssn/Property"/>
        <ssn:hasMeasurementProperty rdf:resource="http://http://www.esonetyellowpages.com/vocab/150-Kilo-Hertz"/>
        <ssn:hasProperty rdf:resource="http://http://www.esonetyellowpages.com/vocab/150-Kilo-Hertz"/>
        <ssn:isPropertyOf rdf:resource="http://http://www.esonetyellowpages.com/vocab/E2-M3A-ADCP-WHS-150Khz"/>
        <rdfs:label xml:lang="en">Workhorse Quartermaster 150 kHz ADCP Frequency</rdfs:label>
    </owl:NamedIndividual>
    


    <!-- http://http://www.esonetyellowpages.com/vocab/Workhorse-Quartermaster-150-kHz-ADCP-Max-Profiling-Range -->

    <owl:NamedIndividual rdf:about="http://http://www.esonetyellowpages.com/vocab/Workhorse-Quartermaster-150-kHz-ADCP-Max-Profiling-Range">
        <rdf:type rdf:resource="https://www.w3.org/ns/ssn/MeasurementCapability"/>
        <rdf:type rdf:resource="https://www.w3.org/ns/ssn/Property"/>
        <ssn:hasMeasurementProperty rdf:resource="http://http://www.esonetyellowpages.com/vocab/300-Meter"/>
        <ssn:hasProperty rdf:resource="http://http://www.esonetyellowpages.com/vocab/300-Meter"/>
        <ssn:isPropertyOf rdf:resource="http://http://www.esonetyellowpages.com/vocab/E2-M3A-ADCP-WHS-150Khz"/>
        <rdfs:label xml:lang="en">Workhorse Quartermaster 150 kHz ADCP Max Profiling Range</rdfs:label>
    </owl:NamedIndividual>
    


    <!-- http://http://www.esonetyellowpages.com/vocab/150-Kilo-Hertz -->

    <owl:NamedIndividual rdf:about="http://http://www.esonetyellowpages.com/vocab/150-Kilo-Hertz">
        <rdf:type rdf:resource="http://schema.org/QuantitativeValue"/>
        <rdf:type rdf:resource="https://www.w3.org/ns/ssn/MeasurementFrequency"/>
        <rdf:type rdf:resource="https://www.w3.org/ns/ssn/MeasurementProperty"/>
        <rdf:type rdf:resource="https://www.w3.org/ns/ssn/Property"/>
        <schema:unitCode rdf:resource="http://qudt.org/vocab/unit#KiloHertz"/>
        <ssn:isPropertyOf rdf:resource="http://http://www.esonetyellowpages.com/vocab/Workhorse-Quartermaster-150-kHz-ADCP-Frequency"/>
        <schema:value rdf:datatype="http://www.w3.org/2001/XMLSchema#float">150.0</schema:value>
        <rdfs:label xml:lang="en">150 kilo Hertz</rdfs:label>
    </owl:NamedIndividual>
    


    <!-- http://http://www.esonetyellowpages.com/vocab/300-Meter -->

    <owl:NamedIndividual rdf:about="http://http://www.esonetyellowpages.com/vocab/300-Meter">
        <rdf:type rdf:resource="http://schema.org/QuantitativeValue"/>
        <rdf:type rdf:resource="https://www.w3.org/ns/ssn/MeasurementProperty"/>
        <rdf:type rdf:resource="https://www.w3.org/ns/ssn/MeasurementRange"/>
        <rdf:type rdf:resource="https://www.w3.org/ns/ssn/Property"/>
        <schema:unitCode rdf:resource="http://qudt.org/vocab/unit#Meter"/>
        <ssn:isPropertyOf rdf:resource="http://http://www.esonetyellowpages.com/vocab/Workhorse-Quartermaster-150-kHz-ADCP-Max-Profiling-Range"/>
        <schema:value rdf:datatype="http://www.w3.org/2001/XMLSchema#float">300.0</schema:value>
        <rdfs:label xml:lang="en">300 Meter</rdfs:label>
    </owl:NamedIndividual>
    


    <!-- http://qudt.org/vocab/unit#KiloHertz -->

    <owl:NamedIndividual rdf:about="http://qudt.org/vocab/unit#KiloHertz"/>
    


    <!-- http://qudt.org/vocab/unit#Meter -->

    <owl:NamedIndividual rdf:about="http://qudt.org/vocab/unit#Meter"/>
    


    <!-- 
    ///////////////////////////////////////////////////////////////////////////////////////
    //
    // Annotations
    //
    ///////////////////////////////////////////////////////////////////////////////////////
     -->

    <rdf:Description rdf:about="https://www.w3.org/ns/ssn/SensorDataSheet">
        <rdfs:comment>A data sheet records properties of a sensor.  A data sheet might describe for example the accuracy in various conditions, the power use, the types of connectors that the sensor has, etc.  

Generally a sensor&apos;s properties are recorded directly (with hasMeasurementCapability, for example), but the data sheet can be used for example to record the manufacturers specifications verses observed capabilites, or if more is known than the manufacturer specifies, etc.  The data sheet is an information object about the sensor&apos;s properties, rather than a direct link to the actual properties themselves.</rdfs:comment>
        <rdfs:label>Sensor Data Sheet</rdfs:label>
    </rdf:Description>
</rdf:RDF>



<!-- Generated by the OWL API (version 4.2.1.20160306-0033) https://github.com/owlcs/owlapi -->

